src/Eqvivalence/BsFs/BX5Eqvivalence.v
@@ -52,87 +52,6 @@ Import BigStep.
 
 
 
-(*
-  Greek Letters:
-  α β γ δ ε ζ η θ ι κ λ μ ν ξ ο π ρ σ τ υ φ χ ψ ω
-  Α Β Γ Δ Ε Ζ Η Θ Ι Κ Λ Μ Ν Ξ Ο Π Ρ Σ Τ Υ Φ Χ Ψ Ω
-
-  Mathematical Symbols:
-  ∀ ∃ ∈ ∉ ∋ ∌ ∅ ∆ ∇ ∈ ∉ ∋ ∌ ∏ ∑ − ∓ ∗ ∘ ∙ √ ∝ ∞
-  ∧ ∨ ∩ ∪ ∫ ∴ ∵ ∷ ≠ ≡ ≤ ≥ ⊂ ⊃ ⊆ ⊇ ⊕ ⊗ ⊥ ⋂ ⋃ ⌈ ⌉ ⌊ ⌋ ⟨ ⟩
-
-  Superscripts:
-  ⁰ ¹ ² ³ ⁴ ⁵ ⁶ ⁷ ⁸ ⁹ ⁺ ⁻ ⁼ ⁽ ⁾
-  ᵃ ᵇ ᶜ ᵈ ᵉ ᶠ ᵍ ʰ ⁱ ʲ ᵏ ˡ ᵐ ⁿ ᵒ ᵖ ʳ ˢ ᵗ ᵘ ᵛ ʷ ˣ ʸ ᶻ
-  ᴬ ᴮ ᴰ ᴱ ᴳ ᴴ ᴵ ᴶ ᴷ ᴸ ᴹ ᴺ ᴼ ᴾ ᴿ ᵀ ᵁ ᵂ
-
-  Subscripts:
-  ₀ ₁ ₂ ₃ ₄ ₅ ₆ ₇ ₈ ₉ ₊ ₋ ₌ ₍ ₎
-  ₐ ₑ ᵦ ᵧ ᵨ ₓ ₔ ₕ ᵢ ⱼ ₖ ₗ ₘ ₙ ₒ ₚ ᵩ ᵪ
-
-  Arrows:
-  ← ↑ → ↓ ↔ ↕ ⇐ ⇑ ⇒ ⇓ ⇔ ⇕
-
-  Miscellaneous Symbols:
-  © ® ™ ¶ § † ‡ • ‣ ′ ″ ‴ ‵ ‶ ‷ 
-  ‖ ‗ ‾ ‿ ⁀ ⁂ ⁃ ⁄ ⁅ ⁆ 
-  ⁇ ⁈ ⁉ ⁎ ⁏ ⁐ ⁑ ⁒ ⁓ ⁔ ⁕ 
-  ⁖ ⁗ ⁘ ⁙ ⁚ ⁛ ⁜ ⁝ ⁞
-
-
-
-  □ ▢ ▣ ▤ ▥ ▦ ▧ ▨ ▩ ▪ ▫ ▬ ▭ ▮ ▯
-▲ △ ▴ ▵ ▶ ▷ ▸ ▹ ► ▻ ▼ ▽ ▾ ▿ ◀ ◁ ◂ ◃ ◄ ◅
-◆ ◇ ◈ ◉ ◊ ○ ◌ ◍ ◎ ● ◐ ◑ ◒ ◓ ◔ ◕ ◖ ◗
-◘ ◙ ◚ ◛ ◜ ◝ ◞ ◟ ◠ ◡ ◢ ◣ ◤ ◥ ◦ ◧ ◨ ◩ ◪ ◫ ◬ ◭ ◮ ◯
-◰ ◱ ◲ ◳ ◴ ◵ ◶ ◷ ◸ ◹ ◺ ◻ ◼ ◽ ◾ ◿
-Mathematical Symbols:
-∀ ∁ ∂ ∃ ∄ ∅ ∆ ∇ ∈ ∉ ∊ ∋ ∌ ∍ ∎ ∏ ∐ ∑ − ∓ ∔ ∕ ∖ ∗ ∘ ∙ √ ∛ ∜ ∝ ∞
-∟ ∠ ∡ ∢ ∣ ∤ ∥ ∦ ∧ ∨ ∩ ∪ ∫ ∬ ∭ ∮ ∯ ∰ ∱ ∲ ∳ ∴ ∵ ∶ ∷ ∸ ∹ ∺ ∻ ∼ ∽ ∾ ∿
-≀ ≁ ≂ ≃ ≄ ≅ ≆ ≇ ≈ ≉ ≊ ≋ ≌ ≍ ≎ ≏ ≐ ≑ ≒ ≓ ≔ ≕ ≖ ≗ ≘ ≙ ≚ ≛ ≜ ≝ ≞ ≟
-≠ ≡ ≤ ≥ ≦ ≧ ≨ ≩ ≪ ≫ ≬ ≭ ≮ ≯ ≰ ≱ ≲ ≳ ≴ ≵ ≶ ≷ ≸ ≹ ≺ ≻ ≼ ≽ ≾ ≿
-⊀ ⊁ ⊂ ⊃ ⊄ ⊅ ⊆ ⊇ ⊈ ⊉ ⊊ ⊋ ⊌ ⊍ ⊎ ⊏ ⊐ ⊑ ⊒ ⊓ ⊔ ⊕ ⊖ ⊗ ⊘ ⊙ ⊚ ⊛ ⊜ ⊝ ⊞ ⊟ ⊠ ⊡ ⊢ ⊣ ⊤ ⊥ ⊦ ⊧ ⊨ ⊩ ⊪ ⊫ ⊬ ⊭ ⊮ ⊯ ⊰ ⊱ ⊲ ⊳ ⊴ ⊵ ⊶ ⊷ ⊸ ⊹ ⊺ ⊻ ⊼ ⊽ ⊾ ⊿
-⋀ ⋁ ⋂ ⋃ ⋄ ⋅ ⋆ ⋇ ⋈ ⋉ ⋊ ⋋ ⋌ ⋍ ⋎ ⋏ ⋐ ⋑ ⋒ ⋓ ⋔ ⋕ ⋖ ⋗ ⋘ ⋙ ⋚ ⋛ ⋜ ⋝ ⋞ ⋟ ⋠ ⋡ ⋢ ⋣ ⋤ ⋥ ⋦ ⋧ ⋨ ⋩ ⋪ ⋫ ⋬ ⋭ ⋮ ⋯ ⋰ ⋱ ⋲ ⋳ ⋴ ⋵ ⋶ ⋷ ⋸ ⋹ ⋺ ⋻ ⋼ ⋽ ⋾ ⋿
-Currency Symbols:
-¢ £ ¥ € ₣ ₤ ₧ ₨ ₩ ₪ ₫ ₭ ₮ ₯ ₹ ₺ ₼ ₽
-Miscellaneous Symbols:
-☀ ☁ ☂ ☃ ☄ ★ ☆ ☇ ☈ ☉ ☊ ☋ ☌ ☍ ☎ ☏ ☐ ☑ ☒ ☓ ☔ ☕ ☖ ☗ ☘ ☙ ☚ ☛ ☜ ☝ ☞ ☟ ☠ ☡ ☢ ☣ ☤ ☥ ☦ ☧ ☨ ☩ ☪ ☫ ☬ ☭ ☮ ☯ ☰ ☱ ☲ ☳ ☴ ☵ ☶ ☷
-☸ ☹ ☺ ☻ ☼ ☽ ☾ ☿ ♀ ♁ ♂ ♃ ♄ ♅ ♆ ♇ ♈ ♉ ♊ ♋ ♌ ♍ ♎ ♏ ♐ ♑ ♒ ♓ ♔ ♕ ♖ ♗ ♘ ♙ ♚ ♛ ♜ ♝ ♞ ♟ ♠ ♡ ♢ ♣ ♤ ♥ ♦ ♧ ♨ ♩ ♪ ♫ ♬ ♭ ♮ ♯
-✁ ✂ ✃ ✄ ✅ ✆ ✇ ✈ ✉ ✊ ✋ ✌ ✍ ✎ ✏ ✐ ✑ ✒ ✓ ✔ ✕ ✖ ✗ ✘ ✙ ✚ ✛ ✜ ✝ ✞ ✟ ✠ ✡ ✢ ✣ ✤ ✥ ✦ ✧ ✩ ✪ ✫ ✬ ✭ ✮ ✯ ✰ ✱ ✲ ✳ ✴ ✵ ✶ ✷ ✸ ✹ ✺ ✻ ✼ ✽ ✾ ✿ ❀ ❁ ❂ ❃ ❄ ❅ ❆ ❇ ❈ ❉ ❊ ❋ ❌ ❍ ❎ ❏ ❐ ❑ ❒ ❖ ❘ ❙ ❚ ❛ ❜ ❝ ❞ ❢ ❣ ❤ ❥ ❦ ❧
-➔ ➕ ➖ ➗ ➘ ➙ ➚ ➛ ➜ ➝ ➞ ➟ ➠ ➡ ➢ ➣ ➤ ➥ ➦ ➧ ➨ ➩ ➪ ➫ ➬ ➭ ➮ ➯ ➰ ➱ ➲ ➳ ➴ ➵ ➶ ➷ ➸ ➹ ➺ ➻ ➼ ➽ ➾ ➿
-Parentheses and Brackets:
-⦀ ⦁ ⦂ ⦃ ⦄ ⦅ ⦆ ⦇ ⦈ ⦉ ⦊ ⦋ ⦌ ⦍ ⦎ ⦏ ⦐ ⦑ ⦒ ⦓ ⦔ ⦕ ⦖ ⦗ ⦘ ⦙ ⦚ ⦛ ⦜ ⦝ ⦞ ⦟ ⦠ ⦡ ⦢ ⦣ ⦤ ⦥ ⦦ ⦧ ⦨ ⦩ ⦪ ⦫ ⦬ ⦭ ⦮ ⦯ ⦰ ⦱ ⦲ ⦳ ⦴ ⦵ ⦶ ⦷ ⦸ ⦹ ⦺ ⦻ ⦼ ⦽ ⦾ ⦿
-Combining Diacritical Marks:
-̀ ́ ̂ ̃ ̄ ̅ ̆ ̇ ̈ ̉ ̊ ̋ ̌ ̍ ̎ ̏ ̐ ̑ ̒ ̓ ̔ ̕ ̖ ̗ ̘ ̙ ̚ ̛ ̜ ̝ ̞ ̟ ̠ ̡ ̢ ̣ ̤ ̥ ̦ ̧ ̨ ̩ ̪ ̫ ̬ ̭ ̮ ̯ ̰ ̱ ̲ ̳ ̴ ̵ ̶ ̷ ̸ ̹ ̺ ̻ ̼ ̽ ̾ ̿
-
-
-
-Additional Mathematical Symbols:
-∂ ∆ ∇ ∈ ∉ ∋ ∌ ∍ ∎ ∏ ∐ ∑ − ∓ ∔ ∕ ∖ ∗ ∘ ∙ √ ∛ ∜ ∝ ∞ ∟ ∠ ∡ ∢ ∣ ∤ ∥ ∦ ∧ ∨ ∩ ∪ ∫ ∬ ∭ ∮ ∯ ∰ ∱ ∲ ∳ ∴ ∵ ∶ ∷ ∸ ∹ ∺ ∻ ∼ ∽ ∾ ∿ ≀ ≁ ≂ ≃ ≄ ≅ ≆ ≇ ≈ ≉ ≊ ≋ ≌ ≍ ≎ ≏ ≐ ≑ ≒ ≓ ≔ ≕ ≖ ≗ ≘ ≙ ≚ ≛ ≜ ≝ ≞ ≟ ≠ ≡ ≤ ≥ ≦ ≧ ≨ ≩ ≪ ≫ ≬ ≭ ≮ ≯ ≰ ≱ ≲ ≳ ≴ ≵ ≶ ≷ ≸ ≹ ≺ ≻ ≼ ≽ ≾ ≿ ⊀ ⊁ ⊂ ⊃ ⊄ ⊅ ⊆ ⊇ ⊈ ⊉ ⊊ ⊋ ⊌ ⊍ ⊎ ⊏ ⊐ ⊑ ⊒ ⊓ ⊔ ⊕ ⊖ ⊗ ⊘ ⊙ ⊚ ⊛ ⊜ ⊝ ⊞ ⊟ ⊠ ⊡ ⊢ ⊣ ⊤ ⊥ ⊦ ⊧ ⊨ ⊩ ⊪ ⊫ ⊬ ⊭ ⊮ ⊯ ⊰ ⊱ ⊲ ⊳ ⊴ ⊵ ⊶ ⊷ ⊸ ⊹ ⊺ ⊻ ⊼ ⊽ ⊾ ⊿ ⋀ ⋁ ⋂ ⋃ ⋄ ⋅ ⋆ ⋇ ⋈ ⋉ ⋊ ⋋ ⋌ ⋍ ⋎ ⋏ ⋐ ⋑ ⋒ ⋓ ⋔ ⋕ ⋖ ⋗ ⋘ ⋙ ⋚ ⋛ ⋜ ⋝ ⋞ ⋟ ⋠ ⋡ ⋢ ⋣ ⋤ ⋥ ⋦ ⋧ ⋨ ⋩ ⋪ ⋫ ⋬ ⋭ ⋮ ⋯ ⋰ ⋱ ⋲ ⋳ ⋴ ⋵ ⋶ ⋷ ⋸ ⋹ ⋺ ⋻ ⋼ ⋽ ⋾ ⋿
-Additional Arrows:
-← ↑ → ↓ ↔ ↕ ⇐ ⇑ ⇒ ⇓ ⇔ ⇕ ⇖ ⇗ ⇘ ⇙ ⇚ ⇛ ⇜ ⇝ ⇞ ⇟ ⇠ ⇡ ⇢ ⇣ ⇤ ⇥ ⇦ ⇧ ⇨ ⇩ ⇪ ⇫ ⇬ ⇭ ⇮ ⇯ ⇰ ⇱ ⇲ ⇳ ⇴ ⇵ ⇶ ⇷ ⇸ ⇹ ⇺ ⇻ ⇼ ⇽ ⇾ ⇿
-Additional Geometric Shapes:
-◀ ◁ ◂ ◃ ◄ ◅ ◆ ◇ ◈ ◉ ◊ ○ ◌ ◍ ◎ ● ◐ ◑ ◒ ◓ ◔ ◕ ◖ ◗ ◘ ◙ ◚ ◛ ◜ ◝ ◞ ◟ ◠ ◡ ◢ ◣ ◤ ◥ ◦ ◧ ◨ ◩ ◪ ◫ ◬ ◭ ◮ ◯ ◰ ◱ ◲ ◳ ◴ ◵ ◶ ◷ ◸ ◹ ◺ ◻ ◼ ◽ ◾ ◿
-Additional Parentheses and Brackets:
-⦀ ⦁ ⦂ ⦃ ⦄ ⦅ ⦆ ⦇ ⦈ ⦉ ⦊ ⦋ ⦌ ⦍ ⦎ ⦏ ⦐ ⦑ ⦒ ⦓ ⦔ ⦕ ⦖ ⦗ ⦘ ⦙ ⦚ ⦛ ⦜ ⦝ ⦞ ⦟ ⦠ ⦡ ⦢ ⦣ ⦤ ⦥ ⦦ ⦧ ⦨ ⦩ ⦪ ⦫ ⦬ ⦭ ⦮ ⦯ ⦰ ⦱ ⦲ ⦳ ⦴ ⦵ ⦶ ⦷ ⦸ ⦹ ⦺ ⦻ ⦼ ⦽ ⦾ ⦿
-Additional Currency Symbols:
-¢ £ ¥ € ₣ ₤ ₧ ₨ ₩ ₪ ₫ ₭ ₮ ₯ ₹ ₺ ₼ ₽
-Additional Miscellaneous Symbols:
-☀ ☁ ☂ ☃ ☄ ★ ☆ ☇ ☈ ☉ ☊ ☋ ☌ ☍ ☎ ☏ ☐ ☑ ☒ ☓ ☔ ☕ ☖ ☗ ☘ ☙ ☚ ☛ ☜ ☝ ☞ ☟ ☠ ☡ ☢ ☣ ☤ ☥ ☦ ☧ ☨ ☩ ☪ ☫ ☬ ☭ ☮ ☯ ☰ ☱ ☲ ☳ ☴ ☵ ☶ ☷ ☸ ☹ ☺ ☻ ☼ ☽ ☾ ☿ ♀ ♁ ♂ ♃ ♄ ♅ ♆ ♇ ♈ ♉ ♊ ♋ ♌ ♍ ♎ ♏ ♐ ♑ ♒ ♓ ♔ ♕ ♖ ♗ ♘ ♙ ♚ ♛ ♜ ♝ ♞ ♟ ♠ ♡ ♢ ♣ ♤ ♥ ♦ ♧ ♨ ♩ ♪ ♫ ♬ ♭ ♮ ♯ ✁ ✂ ✃ ✄ ✅ ✆ ✇ ✈ ✉ ✊ ✋ ✌ ✍ ✎ ✏ ✐ ✑ ✒ ✓ ✔ ✕ ✖ ✗ ✘ ✙ ✚ ✛ ✜ ✝ ✞ ✟ ✠ ✡ ✢ ✣ ✤ ✥ ✦ ✧ ✩ ✪ ✫ ✬ ✭ ✮ ✯ ✰ ✱ ✲ ✳ ✴ ✵ ✶ ✷ ✸ ✹ ✺ ✻ ✼ ✽ ✾ ✿ ❀ ❁ ❂ ❃ ❄ ❅ ❆ ❇ ❈ ❉ ❊ ❋ ❌ ❍ ❎ ❏ ❐ ❑ ❒ ❖ ❘ ❙ ❚ ❛ ❜ ❝ ❞ ❢ ❣ ❤ ❥ ❦ ❧ ➔ ➕ ➖ ➗ ➘ ➙ ➚ ➛ ➜ ➝ ➞ ➟ ➠ ➡ ➢ ➣ ➤ ➥ ➦ ➧ ➨ ➩ ➪ ➫ ➬ ➭ ➮ ➯ ➰ ➱ ➲ ➳ ➴ ➵ ➶ ➷ ➸ ➹ ➺ ➻ ➼ ➽ ➾ ➿
-Additional Combining Diacritical Marks:
-̀ ́ ̂ ̃ ̄ ̅ ̆ ̇ ̈ ̉ ̊ ̋ ̌ ̍ ̎ ̏ ̐ ̑ ̒ ̓ ̔ ̕ ̖ ̗ ̘ ̙ ̚ ̛ ̜ ̝ ̞ ̟ ̠ ̡ ̢ ̣ ̤ ̥ ̦ ̧ ̨ ̩ ̪ ̫ ̬ ̭ ̮ ̯ ̰ ̱ ̲ ̳ ̴ ̵ ̶ ̷ ̸ ̹ ̺ ̻ ̼ ̽ ̾ ̿
-Additional Superscripts and Subscripts:
-⁰ ¹ ² ³ ⁴ ⁵ ⁶ ⁷ ⁸ ⁹ ⁺ ⁻ ⁼ ⁽ ⁾ ᵃ ᵇ ᶜ ᵈ ᵉ ᶠ ᵍ ʰ ⁱ ʲ ᵏ ˡ ᵐ ⁿ ᵒ ᵖ ʳ ˢ ᵗ ᵘ ᵛ ʷ ˣ ʸ ᶻ ᴬ ᴮ ᴰ ᴱ ᴳ ᴴ ᴵ ᴶ ᴷ ᴸ ᴹ ᴺ ᴼ ᴾ ᴿ ᵀ ᵁ ᵂ ₀ ₁ ₂ ₃ ₄ ₅ ₆ ₇ ₈ ₉ ₊ ₋ ₌ ₍ ₎ ₐ ₑ ᵦ ᵧ ᵨ ₓ ₔ ₕ ᵢ ⱼ ₖ ₗ ₘ ₙ ₒ ₚ ᵩ ᵪ
-Additional Arrows and Miscellaneous Symbols:
-← ↑ → ↓ ↔ ↕ ⇐ ⇑ ⇒ ⇓ ⇔ ⇕ ⇖ ⇗ ⇘ ⇙ ⇚ ⇛ ⇜ ⇝ ⇞ ⇟ ⇠ ⇡ ⇢ ⇣ ⇤ ⇥ ⇦ ⇧ ⇨ ⇩ ⇪ ⇫ ⇬ ⇭ ⇮ ⇯ ⇰ ⇱ ⇲ ⇳ ⇴ ⇵ ⇶ ⇷ ⇸ ⇹ ⇺ ⇻ ⇼ ⇽ ⇾ ⇿
-
-**)
-
-
-
-
-
-
 
 
 
@@ -153,6 +72,10 @@ Section ENil.
 
 
 
+(*
+⟨ [], ᴱ′(δₑᶠ(ᵉ[]ᴮ ⇓ Γ)) ⟩ -->* ᵛˢ′(δᵥₗᶠ([ᵛ[]ᴮ]))
+
+*)
   Theorem eq_bsfs_enil_to_vnil :
     forall Γ,
       ⟨ [], erase_names Γ ENil ⟩ -->* erase_valseq [VNil].
@@ -176,17 +99,19 @@ Section ELit.
 
 
 
+(*
+⟨ [], ᴱ′(δₑᶠ(ᵉᴸlᴮᴮ ⇓ Γ)) ⟩ -->* ᵛˢ′(δᵥₗᶠ([ᵛᴸlᴮᴮ]))
+*)
   Theorem eq_bsfs_elit_to_vlit :
-    forall Γ litᴮ ,
-      ⟨ [], erase_names Γ (ELit litᴮ) ⟩ -->* erase_valseq [VLit litᴮ].
+    forall Γ lᴮ ,
+      ⟨ [], erase_names Γ (ELit lᴮ) ⟩ -->* erase_valseq [VLit lᴮ].
   Proof.
     itr.
     (* #1 Unfold Converters: simpl *)
     smp.
     (* #2 Convert Syntax from BigStep to FrameStack: remember *)
-    rem - litᶠ as Hlit:
-      (convert_lit litᴮ);
-      clr - Hlit litᴮ Γ.
+    rem - lᶠ as Hl / Hl lᴮ Γ:
+      (convert_lit lᴮ).
     (* #3 FrameStack Evaluation: open/step *)
     open.
     step.
@@ -221,7 +146,12 @@ End ELit.
 Section EVar.
 
 
-
+(*
+Hget : Γ[↤ xᴮ] = Some [vᴮ]
+Hscp : VALCLOSED δᵥᶠ(vᴮ)
+______________________________________(1/1)
+⟨ [], ᴱ′(δₑᶠ(ᵉˣxᴮᴮ ⇓ Γ)) ⟩ -->* ᵛˢ′(δᵥₗᶠ([vᴮ]))
+*)
   Theorem eq_bsfs_evar_to_value :
     forall Γ xᴮ vᴮ,
         get_value Γ (inl xᴮ) = Some [vᴮ]
@@ -279,6 +209,12 @@ Section EFunId.
 
 
 
+(*
+Hget : Γ[fᴮ ↦] = Some [vᴮ]
+Hscp : VALCLOSED δᵥᶠ(vᴮ)
+______________________________________(1/1)
+⟨ [], ᴱ′(δₑᶠ(ᵉᶠfᴮᴮ ⇓ Γ)) ⟩ -->* ᵛˢ′(δᵥₗᶠ([vᴮ]))
+*)
   Theorem eq_bsfs_efunid_to_value :
     forall Γ fᴮ vᴮ,
         get_value Γ (inr fᴮ) = Some [vᴮ]
@@ -349,7 +285,12 @@ End EFunId.
 Section ECons.
 
 
-
+(*
+IHFse_v₁ : ⟨ [], ᴱ′(δₑᶠ(e₁ᴮ ⇓ Γ)) ⟩ -->* ᵛˢ′(δᵥₗᶠ([v₁ᴮ]))
+IHFse_v₂ : ⟨ [], ᴱ′(δₑᶠ(e₂ᴮ ⇓ Γ)) ⟩ -->* ᵛˢ′(δᵥₗᶠ([v₂ᴮ]))
+______________________________________(1/1)
+⟨ [], ᴱ′(δₑᶠ(ᵉ[e₁ᴮ|e₂ᴮ]ᴮ ⇓ Γ)) ⟩ -->* ᵛˢ′(δᵥₗᶠ([ᵛ[v₁ᴮ|v₂ᴮ]ᴮ]))
+*)
   Theorem eq_bsfs_econs_to_vcons :
     forall Γ e₁ᴮ e₂ᴮ v₁ᴮ v₂ᴮ,
         ⟨ [], erase_names Γ e₁ᴮ ⟩ -->* erase_valseq [v₁ᴮ]
@@ -391,6 +332,12 @@ Section ECons.
 
 
 
+(*
+IHFse_q₁ : ⟨ [], ᴱ′(δₑᶠ(e₁ᴮ ⇓ Γ)) ⟩ -->* ᵉˣᶜ′(δₓᶠ(q₁ᴮ))
+IHFse_v₂ : ⟨ [], ᴱ′(δₑᶠ(e₂ᴮ ⇓ Γ)) ⟩ -->* ᵛˢ′(δᵥₗᶠ([v₂ᴮ]))
+______________________________________(1/1)
+⟨ [], ᴱ′(δₑᶠ(ᵉ[e₁ᴮ|e₂ᴮ]ᴮ ⇓ Γ)) ⟩ -->* ᵉˣᶜ′(δₓᶠ(q₁ᴮ))
+*)
   Theorem eq_bsfs_econs_to_exception1 :
     forall Γ e₁ᴮ e₂ᴮ q₁ᴮ v₂ᴮ,
         ⟨ [], erase_names Γ e₁ᴮ ⟩ -->* erase_exc q₁ᴮ
@@ -431,6 +378,11 @@ Section ECons.
 
 
 
+(*
+IHFse_q₂ : ⟨ [], ᴱ′(δₑᶠ(e₂ᴮ ⇓ Γ)) ⟩ -->* ᵉˣᶜ′(δₓᶠ(q₂ᴮ))
+______________________________________(1/1)
+⟨ [], ᴱ′(δₑᶠ(ᵉ[e₁ᴮ|e₂ᴮ]ᴮ ⇓ Γ)) ⟩ -->* ᵉˣᶜ′(δₓᶠ(q₂ᴮ))
+*)
   Theorem eq_bsfs_econs_to_exception2 :
     forall Γ e₁ᴮ e₂ᴮ q₂ᴮ,
         ⟨ [], erase_names Γ e₂ᴮ ⟩ -->* erase_exc q₂ᴮ
@@ -478,6 +430,12 @@ Section ESeq.
 
 
 
+(*
+IHFse_v₁ : ⟨ [], ᴱ′(δₑᶠ(e₁ᴮ ⇓ Γ)) ⟩ -->* ᵛˢ′(δᵥₗᶠ([v₁ᴮ]))
+IHFse_r₂ : ⟨ [], ᴱ′(δₑᶠ(e₂ᴮ ⇓ Γ)) ⟩ -->* δᶠ(r₂ᴮ)
+______________________________________(1/1)
+⟨ [], ᴱ′(δₑᶠ(ᵉdoᴮ e₁ᴮ e₂ᴮ ⇓ Γ)) ⟩ -->* δᶠ(r₂ᴮ)
+*)
   Theorem eq_bsfs_eseq_to_result :
     forall Γ e₁ᴮ e₂ᴮ v₁ᴮ r₂ᴮ,
         ⟨ [], erase_names Γ e₁ᴮ ⟩ -->* erase_valseq [v₁ᴮ]
@@ -517,6 +475,11 @@ Section ESeq.
 
 
 
+(*
+IHFse_q₁ : ⟨ [], ᴱ′(δₑᶠ(e₁ᴮ ⇓ Γ)) ⟩ -->* ᵉˣᶜ′(δₓᶠ(q₁ᴮ))
+______________________________________(1/1)
+⟨ [], ᴱ′(δₑᶠ(ᵉdoᴮ e₁ᴮ e₂ᴮ ⇓ Γ)) ⟩ -->* ᵉˣᶜ′(δₓᶠ(q₁ᴮ))
+*)
   Theorem eq_bsfs_eseq_to_exception :
     forall Γ e₁ᴮ e₂ᴮ q₁ᴮ,
         ⟨ [], erase_names Γ e₁ᴮ ⟩ -->* erase_exc q₁ᴮ
@@ -578,6 +541,11 @@ Section EFun.
 
 
 
+(*
+Hscp : is_result ᵛˢ′(δᵥₗᶠ([ᵛ⟨id : [], xsᴮ, eᴮ, Γ⟩ᴮ]))
+______________________________________(1/1)
+⟨ [], ᴱ′(δₑᶠ(ᵉfunᴮ(xsᴮ) -> eᴮ ⇓ Γ)) ⟩ -->* ᵛˢ′(δᵥₗᶠ([ᵛ⟨id : [], xsᴮ, eᴮ, Γ⟩ᴮ]))
+*)
   Theorem eq_bsfs_efun_to_vclos :
     forall Γ xsᴮ eᴮ id,
         is_result (erase_valseq [VClos Γ [] id xsᴮ eᴮ])
@@ -630,6 +598,11 @@ Section ELetRec.
 
 
 
+(*
+IHFse_r : ⟨ [], ᴱ′(δₑᶠ(eᴮ ⇓ append_funs_to_env extᴮ Γ id)) ⟩ -->* δᶠ(rᴮ)
+______________________________________(1/1)
+⟨ [], ᴱ′(δₑᶠ(ᵉletrecᴮ extᴮ in eᴮ ⇓ Γ)) ⟩ -->* δᶠ(rᴮ)
+*)
   Theorem eq_bsfs_eletrec_to_result :
     forall Γ extᴮ eᴮ id rᴮ,
         ⟨ [], erase_names (append_funs_to_env extᴮ Γ id) eᴮ ⟩ -->*
@@ -719,6 +692,13 @@ Section ELet.
 
 
 
+(*
+Hlen₁ : ˡ|xs₁ᴮ| = ˡ|vs₁ᴮ|
+IHFse_vs₁ : ⟨ [], ᴱ′(δₑᶠ(e₁ᴮ ⇓ Γ)) ⟩ -->* ᵛˢ′(δᵥₗᶠ(vs₁ᴮ))
+IHFse_r₂ : ⟨ [], ᴱ′(δₑᶠ(e₂ᴮ ⇓ append_vars_to_env xs₁ᴮ vs₁ᴮ Γ)) ⟩ -->* δᶠ(r₂ᴮ)
+______________________________________(1/1)
+⟨ [], ᴱ′(δₑᶠ(ᵉletᴮ<xs₁ᴮ> = e₁ᴮ in e₂ᴮ ⇓ Γ)) ⟩ -->* δᶠ(r₂ᴮ)
+*)
   Theorem eq_bsfs_elet_to_result :
     forall Γ xs₁ᴮ e₁ᴮ e₂ᴮ vs₁ᴮ r₂ᴮ,
         length xs₁ᴮ = length vs₁ᴮ
@@ -777,6 +757,11 @@ Section ELet.
 
 
 
+(*
+IHFse_q₁ : ⟨ [], ᴱ′(δₑᶠ(e₁ᴮ ⇓ Γ)) ⟩ -->* ᵉˣᶜ′(δₓᶠ(q₁ᴮ))
+______________________________________(1/1)
+⟨ [], ᴱ′(δₑᶠ(ᵉletᴮ<xs₁ᴮ> = e₁ᴮ in e₂ᴮ ⇓ Γ)) ⟩ -->* ᵉˣᶜ′(δₓᶠ(q₁ᴮ))
+*)
   Theorem eq_bsfs_elet_exception :
     forall Γ xs₁ᴮ e₁ᴮ e₂ᴮ q₁ᴮ,
         ⟨ [], erase_names Γ e₁ᴮ ⟩ -->* erase_exc q₁ᴮ
@@ -831,6 +816,13 @@ Section ETry.
 
 
 
+(*
+Hlen₁ : ˡ|xs₁ᴮ| = ˡ|vs₁ᴮ|
+IHFse_vs₁ : ⟨ [], ᴱ′(δₑᶠ(e₁ᴮ ⇓ Γ)) ⟩ -->* ᵛˢ′(δᵥₗᶠ(vs₁ᴮ))
+IHFse_r₂ : ⟨ [], ᴱ′(δₑᶠ(e₂ᴮ ⇓ append_vars_to_env xs₁ᴮ vs₁ᴮ Γ)) ⟩ -->* δᶠ(r₂ᴮ)
+______________________________________(1/1)
+⟨ [], ᴱ′(δₑᶠ(ᵉtryᴮ e₁ᴮ of <xs₁ᴮ> -> e₂ᴮ catch <xs₂ᴮ> -> e₃ᴮ ⇓ Γ)) ⟩ -->* δᶠ(r₂ᴮ)
+*)
   Theorem eq_bsfs_etry_to_result1 :
     forall Γ xs₁ᴮ xs₂ᴮ e₁ᴮ e₂ᴮ e₃ᴮ vs₁ᴮ r₂ᴮ,
         length xs₁ᴮ = length vs₁ᴮ
@@ -895,6 +887,13 @@ Section ETry.
 
 
 
+(*
+Hlen₂ : ˡ|xs₂ᴮ| = 3
+IHFse_q₁ : ⟨ [], ᴱ′(δₑᶠ(e₁ᴮ ⇓ Γ)) ⟩ -->* ᵉˣᶜ′(δₓᶠ(q₁ᴮ))
+IHFse_r₃ : ⟨ [], ᴱ′(δₑᶠ(e₃ᴮ ⇓ append_vars_to_env xs₂ᴮ (q₁ᴮ ᶻ⇒ᵛˢ) Γ)) ⟩ -->* δᶠ(r₃ᴮ)
+______________________________________(1/1)
+⟨ [], ᴱ′(δₑᶠ(ᵉtryᴮ e₁ᴮ of <xs₁ᴮ> -> e₂ᴮ catch <xs₂ᴮ> -> e₃ᴮ ⇓ Γ)) ⟩ -->* δᶠ(r₃ᴮ)
+*)
   Theorem eq_bsfs_etry_to_result2 :
     forall Γ xs₁ᴮ xs₂ᴮ e₁ᴮ e₂ᴮ e₃ᴮ q₁ᴮ r₃ᴮ,
         length xs₂ᴮ = 3
@@ -989,16 +988,25 @@ Section EValues.
 
 
 
+(*
+Hlen : ˡ|esᴮ| = ˡ|vsᴮ|
+IHFse_nth :
+  ∀ i : nat,
+    i < ˡ|esᴮ|
+    → ⟨ [], ᴱ′(δₑᶠ(nth i esᴮ eₓᴮ ⇓ Γ)) ⟩ -->* ᵛˢ′(δᵥₗᶠ([nth i vsᴮ vₓᴮ]))
+______________________________________(1/1)
+⟨ [], ᴱ′(δₑᶠ(ᵉ<esᴮ>ᴮ ⇓ Γ)) ⟩ -->* ᵛˢ′(δᵥₗᶠ(vsᴮ))
+*)
   Theorem eq_bsfs_evalues_to_valseq :
-    forall Γ elᴮ eₓᴮ vlᴮ vₓᴮ,
-        length elᴮ = length vlᴮ
+    forall Γ esᴮ eₓᴮ vsᴮ vₓᴮ,
+        length esᴮ = length vsᴮ
     ->  (forall i,
-            i < length elᴮ
-        ->  ⟨ [], erase_names Γ (nth i elᴮ eₓᴮ) ⟩ -->* 
-                  erase_valseq [nth i vlᴮ vₓᴮ])
-    ->  ⟨ [], erase_names Γ (EValues elᴮ) ⟩ -->* erase_valseq vlᴮ.
+            i < length esᴮ
+        ->  ⟨ [], erase_names Γ (nth i esᴮ eₓᴮ) ⟩ -->* 
+                  erase_valseq [nth i vsᴮ vₓᴮ])
+    ->  ⟨ [], erase_names Γ (EValues esᴮ) ⟩ -->* erase_valseq vsᴮ.
   Proof.
-    itr - Γ elᴮ eₓᴮ vlᴮ vₓᴮ Hlen IHFse_nth.
+    itr - Γ esᴮ eₓᴮ vsᴮ vₓᴮ Hlen IHFse_nth.
     (* #0 Pre Formalize Hypothesis: rewrite/symmetry *)
     rwr - Hlen in IHFse_nth.
     sym - Hlen.
@@ -1015,27 +1023,27 @@ Section EValues.
     rem - ξ as Heqv_ξ / Heqv_ξ Γ:
           (list_subst (map erase_val' Γ.vals) idsubst).
     psc - fs_eval_nth_map_erase_forall as IHFse_nth':
-          σ ξ elᴮ eₓᴮ vlᴮ vₓᴮ IHFse_nth.
+          σ ξ esᴮ eₓᴮ vsᴮ vₓᴮ IHFse_nth.
           ren - IHFse_nth: IHFse_nth'.
       (* Expressions *)
-    rem - elᶠ eₓᶠ as Heqv_el Heqv_eₓ / Heqv_eₓ eₓᴮ:
-          (map (fun e => (erase_exp σ e).[ξ]) elᴮ)
+    rem - esᶠ eₓᶠ as Heqv_es Heqv_eₓ / Heqv_eₓ eₓᴮ:
+          (map (fun e => (erase_exp σ e).[ξ]) esᴮ)
           ((erase_exp σ eₓᴮ).[ξ]).
     erewrite length_map_erase_exp_eq in *.
-          2: exa - Heqv_el.
-          clr - Heqv_el elᴮ σ ξ.
+          2: exa - Heqv_es.
+          clr - Heqv_es esᴮ σ ξ.
       (* Values *)
-    rem - vlᶠ vₓᶠ as Heqv_vl Heqv_vₓ / Heqv_vₓ vₓᴮ:
-          (map erase_val' vlᴮ)
+    rem - vsᶠ vₓᶠ as Heqv_vs Heqv_vₓ / Heqv_vₓ vₓᴮ:
+          (map erase_val' vsᴮ)
           (erase_val' vₓᴮ).
     erewrite length_map_erase_val_eq in *.
-          2-3: exa - Heqv_vl.
-          clr - Heqv_vl vlᴮ.
+          2-3: exa - Heqv_vs.
+          clr - Heqv_vs vsᴮ.
     (* #3 Scope From Nth: pose *)
     pse - fs_eval_nth_to_scope as Hscp:
-          elᶠ eₓᶠ vlᶠ vₓᶠ Hlen IHFse_nth.
+          esᶠ eₓᶠ vsᶠ vₓᶠ Hlen IHFse_nth.
     (* #4 Destruct on Expression List and Solve Empty Branch: destruct *)
-    des - elᶠ as [| e₁ᶠ elᶠ].
+    des - esᶠ as [| e₁ᶠ esᶠ].
     { (* - Empty List Branch *)
           clr - IHFse_nth Hscp eₓᶠ vₓᶠ.
           (* #4.1 Both List Empty: apply/subst *)
@@ -1046,28 +1054,28 @@ Section EValues.
           step.
     } (* - Cons List Branch *)
     (* #5 Both List Cons: destruct + inversion/subst *)
-    des - vlᶠ as [| v₁ᶠ vlᶠ]:
+    des - vsᶠ as [| v₁ᶠ vsᶠ]:
           ivs - Hlen.
     (* #6 Pose Nth Cons Theorem: pose/destruct *)
     psc - fs_eval_nth_cons as IHFse_nth_cons:
-          e₁ᶠ elᶠ eₓᶠ v₁ᶠ vlᶠ vₓᶠ IHFse_nth.
+          e₁ᶠ esᶠ eₓᶠ v₁ᶠ vsᶠ vₓᶠ IHFse_nth.
     des - IHFse_nth_cons as [IHFse_v₁ IHFse_nth].
     (* #7 Pose From Nth to Result: apply/pose *)
-    app - length_cons in Hlen.
+    app - length_cons_eq in Hlen.
     pose proof create_result_ivalues
-          v₁ᶠ vlᶠ [] as Hcrt.
+          v₁ᶠ vsᶠ [] as Hcrt.
     pose proof fs_eval_nth_to_result
-          IValues elᶠ eₓᶠ [] v₁ᶠ vlᶠ vₓᶠ (RValSeq (v₁ᶠ :: vlᶠ))
+          IValues esᶠ eₓᶠ [] v₁ᶠ vsᶠ vₓᶠ (RValSeq (v₁ᶠ :: vsᶠ))
           [] [] Hlen Hcrt IHFse_nth
-          as IHFse_vl.
+          as IHFse_vs.
     clr - Hlen Hcrt IHFse_nth eₓᶠ vₓᶠ.
     (* #8 Destruct Inductive Hypothesis: destruct *)
     des - IHFse_v₁ as [k_v₁ [_ Hstp_v₁]].
-    des - IHFse_vl as [k_vl    Hstp_vl].
+    des - IHFse_vs as [k_vs    Hstp_vs].
     (* #9 FrameStack Evaluation: open/step *)
     open / Hscp.
     step - Hstp_v₁ / e₁ᶠ k_v₁.
-    step - Hstp_vl.
+    step - Hstp_vs.
   Qed.
 
 
@@ -1075,17 +1083,27 @@ Section EValues.
 
 
 
+(*
+Hlen : ˡ|vsᴮ| < ˡ|esᴮ|
+IHFse_nth :
+  ∀ i : nat,
+    i < ˡ|vsᴮ|
+    → ⟨ [], ᴱ′(δₑᶠ(nth i esᴮ eₓᴮ ⇓ Γ)) ⟩ -->* ᵛˢ′(δᵥₗᶠ([nth i vsᴮ vₓᴮ]))
+IHFse_qₖ : ⟨ [], ᴱ′(δₑᶠ(nth ˡ|vsᴮ| esᴮ eₓᴮ ⇓ Γ)) ⟩ -->* ᵉˣᶜ′(δₓᶠ(qₖᴮ))
+______________________________________(1/1)
+⟨ [], ᴱ′(δₑᶠ(ᵉ<esᴮ>ᴮ ⇓ Γ)) ⟩ -->* ᵉˣᶜ′(δₓᶠ(qₖᴮ))
+*)
   Theorem eq_bsfs_evalues_to_exception :
-    forall Γ elᴮ eₓᴮ vlᴮ vₓᴮ qₖᴮ,
-        length vlᴮ < length elᴮ
+    forall Γ esᴮ eₓᴮ vsᴮ vₓᴮ qₖᴮ,
+        length vsᴮ < length esᴮ
     ->  (forall i,
-            i < length vlᴮ
-        ->  ⟨ [], erase_names Γ (nth i elᴮ eₓᴮ) ⟩ -->*
-                  erase_valseq [nth i vlᴮ vₓᴮ])
-    ->  ⟨ [], erase_names Γ (nth (length vlᴮ) elᴮ eₓᴮ) ⟩ -->* erase_exc qₖᴮ
-    ->  ⟨ [], erase_names Γ (EValues elᴮ) ⟩ -->* erase_exc qₖᴮ.
+            i < length vsᴮ
+        ->  ⟨ [], erase_names Γ (nth i esᴮ eₓᴮ) ⟩ -->*
+                  erase_valseq [nth i vsᴮ vₓᴮ])
+    ->  ⟨ [], erase_names Γ (nth (length vsᴮ) esᴮ eₓᴮ) ⟩ -->* erase_exc qₖᴮ
+    ->  ⟨ [], erase_names Γ (EValues esᴮ) ⟩ -->* erase_exc qₖᴮ.
   Proof.
-    itr - Γ elᴮ eₓᴮ vlᴮ vₓᴮ qₖᴮ Hlen IHFse_nth IHFse_qₖ.
+    itr - Γ esᴮ eₓᴮ vsᴮ vₓᴮ qₖᴮ Hlen IHFse_nth IHFse_qₖ.
     (* #1 Unfold Converters: simpl/unfold/rewrite *)
     smp.
     ufl - erase_names in *.
@@ -1098,35 +1116,35 @@ Section EValues.
     rem - ξ as Heqv_ξ / Heqv_ξ Γ:
           (list_subst (map erase_val' Γ.vals) idsubst).
     psc - fs_eval_nth_map_erase_forall as IHFse_nth':
-          σ ξ elᴮ eₓᴮ vlᴮ vₓᴮ IHFse_nth;
+          σ ξ esᴮ eₓᴮ vsᴮ vₓᴮ IHFse_nth;
           ren - IHFse_nth: IHFse_nth'.
     rwr - fs_eval_nth_map_erase_single in IHFse_qₖ.
       (* Expressions *)
-    rem - elᶠ eₓᶠ as Heqv_el Heqv_eₓ / Heqv_eₓ eₓᴮ:
-          (map (fun e => (erase_exp σ e).[ξ]) elᴮ)
+    rem - esᶠ eₓᶠ as Heqv_es Heqv_eₓ / Heqv_eₓ eₓᴮ:
+          (map (fun e => (erase_exp σ e).[ξ]) esᴮ)
           ((erase_exp σ eₓᴮ).[ξ]).
     erewrite length_map_erase_exp_eq in *.
-          2: exa - Heqv_el.
-          clr - Heqv_el elᴮ σ ξ.
+          2: exa - Heqv_es.
+          clr - Heqv_es esᴮ σ ξ.
     (*Value*)
-    rem - vlᶠ vₓᶠ qₖᶠ as Heqv_vl Heqv_vₓ Heqv_qₖ / Heqv_vₓ Heqv_qₖ vₓᴮ qₖᴮ:
-          (map erase_val' vlᴮ)
+    rem - vsᶠ vₓᶠ qₖᶠ as Heqv_vs Heqv_vₓ Heqv_qₖ / Heqv_vₓ Heqv_qₖ vₓᴮ qₖᴮ:
+          (map erase_val' vsᴮ)
           (erase_val' vₓᴮ)
           (erase_exc qₖᴮ).
     erewrite length_map_erase_val_eq in *.
-          2-4: exa - Heqv_vl.
-          clr - Heqv_vl vlᴮ.
+          2-4: exa - Heqv_vs.
+          clr - Heqv_vs vsᴮ.
     (* #3 Split Expression List: pose/destruct/subst *)
     psc - length_lt_split_middle as Hsplit:
-          Val Exp vlᶠ elᶠ Hlen.
-    des - Hsplit as [el₁ᶠ [eₖᶠ [el₂ᶠ [Hel Hlen]]]].
+          Val Exp vsᶠ esᶠ Hlen.
+    des - Hsplit as [es₁ᶠ [eₖᶠ [es₂ᶠ [Hes Hlen]]]].
     sbt.
     (* #4 Simplify Hypothesis: *)
     rwr - Hlen in IHFse_qₖ.
     smp - IHFse_qₖ.
     rwr - nth_middle in IHFse_qₖ.
     (* #5 Destruct on Expression List and Solve Empty Branch: destruct *)
-    des - el₁ᶠ as [| e₁ᶠ el₁ᶠ].
+    des - es₁ᶠ as [| e₁ᶠ es₁ᶠ].
     { (* - Empty List Branch *)
           clr - IHFse_nth eₓᶠ vₓᶠ.
           (* #5.1 Both List Empty: apply/subst/simpl *)
@@ -1141,29 +1159,29 @@ Section EValues.
           step.
     } (* - Cons List Branch *)
     (* #6 Both List Cons: destruct + inversion/subst *)
-    des - vlᶠ as [| v₁ᶠ vlᶠ]:
+    des - vsᶠ as [| v₁ᶠ vsᶠ]:
           ivs - Hlen.
     (* #7 Pose Nth Cons Theorem: rewrite/pose/destruct *)
-    rewrite cons_app with (l := el₁ᶠ) in IHFse_nth.
+    rewrite cons_app with (l := es₁ᶠ) in IHFse_nth.
     rwl - app_assoc in IHFse_nth.
     do 2 rwl - cons_app in IHFse_nth.
     psc - fs_eval_nth_cons as IHFse_nth_cons:
-          e₁ᶠ (el₁ᶠ ++ eₖᶠ :: el₂ᶠ) eₓᶠ v₁ᶠ vlᶠ vₓᶠ IHFse_nth.
+          e₁ᶠ (es₁ᶠ ++ eₖᶠ :: es₂ᶠ) eₓᶠ v₁ᶠ vsᶠ vₓᶠ IHFse_nth.
     des - IHFse_nth_cons as [IHFse_v₁ IHFse_nth].
     (* #8 Pose From Nth to Result: apply/pose/simple *)
-    app - length_cons in Hlen.
+    app - length_cons_eq in Hlen.
     pose proof fs_eval_nth_to_partial
-          IValues el₁ᶠ eₖᶠ el₂ᶠ eₓᶠ [] v₁ᶠ vlᶠ vₓᶠ Hlen IHFse_nth
-          as IHFse_vl.
+          IValues es₁ᶠ eₖᶠ es₂ᶠ eₓᶠ [] v₁ᶠ vsᶠ vₓᶠ Hlen IHFse_nth
+          as IHFse_vs.
     smp / Hlen IHFse_nth eₓᶠ vₓᶠ.
     (* #9 Destruct Inductive Hypothesis: destruct *)
     des - IHFse_v₁ as [k_v₁  [_      Hstp_v₁]].
-    des - IHFse_vl as [k_vl          Hstp_vl].
+    des - IHFse_vs as [k_vs          Hstp_vs].
     des - IHFse_qₖ as [k_qₖ [Hscp_qₖ Hstp_qₖ]].
     (* #10 FrameStack Evaluation: open/step *)
     open / Hscp_qₖ.
     step - Hstp_v₁ / e₁ᶠ k_v₁.
-    step - Hstp_vl / el₁ᶠ k_vl.
+    step - Hstp_vs / es₁ᶠ k_vs.
     step - Hstp_qₖ / k_qₖ.
     step.
   Qed.
@@ -1184,16 +1202,25 @@ Section ETuple.
 
 
 
+(*
+Hlen : ˡ|esᴮ| = ˡ|vsᴮ|
+IHFse_nth :
+  ∀ i : nat,
+    i < ˡ|esᴮ|
+    → ⟨ [], ᴱ′(δₑᶠ(nth i esᴮ eₓᴮ ⇓ Γ)) ⟩ -->* ᵛˢ′(δᵥₗᶠ([nth i vsᴮ vₓᴮ]))
+______________________________________(1/1)
+⟨ [], ᴱ′(δₑᶠ(ᵉ{esᴮ}ᴮ ⇓ Γ)) ⟩ -->* ᵛˢ′(δᵥₗᶠ([ᵛ{vsᴮ}ᴮ]))
+*)
   Theorem eq_bsfs_etuple_to_vtuple :
-    forall Γ elᴮ eₓᴮ vlᴮ vₓᴮ,
-        length elᴮ = length vlᴮ
+    forall Γ esᴮ eₓᴮ vsᴮ vₓᴮ,
+        length esᴮ = length vsᴮ
     ->  (forall i,
-            i < length elᴮ
-        ->  ⟨ [], erase_names Γ (nth i elᴮ eₓᴮ) ⟩ -->* 
-                  erase_valseq [nth i vlᴮ vₓᴮ])
-    ->  ⟨ [], erase_names Γ (ETuple elᴮ) ⟩ -->* erase_valseq [VTuple vlᴮ].
+            i < length esᴮ
+        ->  ⟨ [], erase_names Γ (nth i esᴮ eₓᴮ) ⟩ -->* 
+                  erase_valseq [nth i vsᴮ vₓᴮ])
+    ->  ⟨ [], erase_names Γ (ETuple esᴮ) ⟩ -->* erase_valseq [VTuple vsᴮ].
   Proof.
-    itr - Γ elᴮ eₓᴮ vlᴮ vₓᴮ Hlen IHFse_nth.
+    itr - Γ esᴮ eₓᴮ vsᴮ vₓᴮ Hlen IHFse_nth.
     (* #0 Pre Formalize Hypothesis: rewrite/symmetry *)
     rwr - Hlen in IHFse_nth.
     sym - Hlen.
@@ -1211,28 +1238,28 @@ Section ETuple.
     rem - ξ as Heqv_ξ / Heqv_ξ Γ:
           (list_subst (map erase_val' Γ.vals) idsubst).
     psc - fs_eval_nth_map_erase_forall as IHFse_nth':
-          σ ξ elᴮ eₓᴮ vlᴮ vₓᴮ IHFse_nth.
+          σ ξ esᴮ eₓᴮ vsᴮ vₓᴮ IHFse_nth.
           ren - IHFse_nth: IHFse_nth'.
       (* Expressions *)
-    rem - elᶠ eₓᶠ as Heqv_el Heqv_eₓ / Heqv_eₓ eₓᴮ:
-          (map (fun e => (erase_exp σ e).[ξ]) elᴮ)
+    rem - esᶠ eₓᶠ as Heqv_es Heqv_eₓ / Heqv_eₓ eₓᴮ:
+          (map (fun e => (erase_exp σ e).[ξ]) esᴮ)
           ((erase_exp σ eₓᴮ).[ξ]).
     erewrite length_map_erase_exp_eq in *.
-          2: exa - Heqv_el.
-          clr - Heqv_el elᴮ σ ξ.
+          2: exa - Heqv_es.
+          clr - Heqv_es esᴮ σ ξ.
       (* Values *)
-    rem - vlᶠ vₓᶠ as Heqv_vl Heqv_vₓ / Heqv_vₓ vₓᴮ:
-          (map erase_val' vlᴮ)
+    rem - vsᶠ vₓᶠ as Heqv_vs Heqv_vₓ / Heqv_vₓ vₓᴮ:
+          (map erase_val' vsᴮ)
           (erase_val' vₓᴮ).
     erewrite length_map_erase_val_eq in *.
-          2-3: exa - Heqv_vl.
-          clr - Heqv_vl vlᴮ.
+          2-3: exa - Heqv_vs.
+          clr - Heqv_vs vsᴮ.
     (* #3 Scope From Nth: pose *)
     pse - fs_eval_nth_to_scope as Hscp':
-          elᶠ eₓᶠ vlᶠ vₓᶠ Hlen IHFse_nth.
-    psc - scope_list_to_tuple as Hscp: vlᶠ Hscp'.
+          esᶠ eₓᶠ vsᶠ vₓᶠ Hlen IHFse_nth.
+    psc - scope_list_to_tuple as Hscp: vsᶠ Hscp'.
     (* #4 Destruct on Expression List and Solve Empty Branch: destruct *)
-    des - elᶠ as [| e₁ᶠ elᶠ].
+    des - esᶠ as [| e₁ᶠ esᶠ].
     { (* - Empty List Branch *)
           clr - IHFse_nth Hscp eₓᶠ vₓᶠ.
           (* #4.1 Both List Empty: apply/subst *)
@@ -1243,28 +1270,28 @@ Section ETuple.
           step.
     } (* - Cons List Branch *)
     (* #5 Both List Cons: destruct + inversion/subst *)
-    des - vlᶠ as [| v₁ᶠ vlᶠ]:
+    des - vsᶠ as [| v₁ᶠ vsᶠ]:
           ivs - Hlen.
     (* #6 Pose Nth Cons Theorem: pose/destruct *)
     psc - fs_eval_nth_cons as IHFse_nth_cons:
-          e₁ᶠ elᶠ eₓᶠ v₁ᶠ vlᶠ vₓᶠ IHFse_nth.
+          e₁ᶠ esᶠ eₓᶠ v₁ᶠ vsᶠ vₓᶠ IHFse_nth.
     des - IHFse_nth_cons as [IHFse_v₁ IHFse_nth].
     (* #7 Pose From Nth to Result: apply/pose *)
-    app - length_cons in Hlen.
+    app - length_cons_eq in Hlen.
     pose proof create_result_ituple
-          v₁ᶠ vlᶠ [] as Hcrt.
+          v₁ᶠ vsᶠ [] as Hcrt.
     pose proof fs_eval_nth_to_result
-          ITuple elᶠ eₓᶠ [] v₁ᶠ vlᶠ vₓᶠ (RValSeq [Syntax.VTuple (v₁ᶠ :: vlᶠ)])
+          ITuple esᶠ eₓᶠ [] v₁ᶠ vsᶠ vₓᶠ (RValSeq [Syntax.VTuple (v₁ᶠ :: vsᶠ)])
           [] [] Hlen Hcrt IHFse_nth
-          as IHFse_vl.
+          as IHFse_vs.
     clr - Hlen Hcrt IHFse_nth eₓᶠ vₓᶠ.
     (* #8 Destruct Inductive Hypothesis: destruct *)
     des - IHFse_v₁ as [k_v₁ [_ Hstp_v₁]].
-    des - IHFse_vl as [k_vl    Hstp_vl].
+    des - IHFse_vs as [k_vs    Hstp_vs].
     (* #9 FrameStack Evaluation: open/step *)
     open / Hscp.
     step - Hstp_v₁ / e₁ᶠ k_v₁.
-    step - Hstp_vl.
+    step - Hstp_vs.
   Qed.
 
 
@@ -1272,17 +1299,27 @@ Section ETuple.
 
 
 
+(*
+Hlen : ˡ|vsᴮ| < ˡ|esᴮ|
+IHFse_nth :
+  ∀ i : nat,
+    i < ˡ|vsᴮ|
+    → ⟨ [], ᴱ′(δₑᶠ(nth i esᴮ eₓᴮ ⇓ Γ)) ⟩ -->* ᵛˢ′(δᵥₗᶠ([nth i vsᴮ vₓᴮ]))
+IHFse_qₖ : ⟨ [], ᴱ′(δₑᶠ(nth ˡ|vsᴮ| esᴮ eₓᴮ ⇓ Γ)) ⟩ -->* ᵉˣᶜ′(δₓᶠ(qₖᴮ))
+______________________________________(1/1)
+⟨ [], ᴱ′(δₑᶠ(ᵉ{esᴮ}ᴮ ⇓ Γ)) ⟩ -->* ᵉˣᶜ′(δₓᶠ(qₖᴮ))
+*)
   Theorem eq_bsfs_etuple_to_exception :
-    forall Γ elᴮ eₓᴮ vlᴮ vₓᴮ qₖᴮ,
-        length vlᴮ < length elᴮ
+    forall Γ esᴮ eₓᴮ vsᴮ vₓᴮ qₖᴮ,
+        length vsᴮ < length esᴮ
     ->  (forall i,
-            i < length vlᴮ
-        ->  ⟨ [], erase_names Γ (nth i elᴮ eₓᴮ) ⟩ -->* 
-                  erase_valseq [nth i vlᴮ vₓᴮ])
-    ->  ⟨ [], erase_names Γ (nth (length vlᴮ) elᴮ eₓᴮ) ⟩ -->* erase_exc qₖᴮ
-    ->  ⟨ [], erase_names Γ (ETuple elᴮ) ⟩ -->* erase_exc qₖᴮ.
+            i < length vsᴮ
+        ->  ⟨ [], erase_names Γ (nth i esᴮ eₓᴮ) ⟩ -->* 
+                  erase_valseq [nth i vsᴮ vₓᴮ])
+    ->  ⟨ [], erase_names Γ (nth (length vsᴮ) esᴮ eₓᴮ) ⟩ -->* erase_exc qₖᴮ
+    ->  ⟨ [], erase_names Γ (ETuple esᴮ) ⟩ -->* erase_exc qₖᴮ.
   Proof.
-    itr - Γ elᴮ eₓᴮ vlᴮ vₓᴮ qₖᴮ Hlen IHFse_nth IHFse_qₖ.
+    itr - Γ esᴮ eₓᴮ vsᴮ vₓᴮ qₖᴮ Hlen IHFse_nth IHFse_qₖ.
     (* #1 Unfold Converters: simpl/unfold/rewrite *)
     smp.
     ufl - erase_names in *.
@@ -1295,35 +1332,35 @@ Section ETuple.
     rem - ξ as Heqv_ξ / Heqv_ξ Γ:
           (list_subst (map erase_val' Γ.vals) idsubst).
     psc - fs_eval_nth_map_erase_forall as IHFse_nth':
-          σ ξ elᴮ eₓᴮ vlᴮ vₓᴮ IHFse_nth;
+          σ ξ esᴮ eₓᴮ vsᴮ vₓᴮ IHFse_nth;
           ren - IHFse_nth: IHFse_nth'.
     rwr - fs_eval_nth_map_erase_single in IHFse_qₖ.
       (* Expressions *)
-    rem - elᶠ eₓᶠ as Heqv_el Heqv_eₓ / Heqv_eₓ eₓᴮ:
-          (map (fun e => (erase_exp σ e).[ξ]) elᴮ)
+    rem - esᶠ eₓᶠ as Heqv_es Heqv_eₓ / Heqv_eₓ eₓᴮ:
+          (map (fun e => (erase_exp σ e).[ξ]) esᴮ)
           ((erase_exp σ eₓᴮ).[ξ]).
     erewrite length_map_erase_exp_eq in *.
-          2: exa - Heqv_el.
-          clr - Heqv_el elᴮ σ ξ.
+          2: exa - Heqv_es.
+          clr - Heqv_es esᴮ σ ξ.
     (*Value*)
-    rem - vlᶠ vₓᶠ qₖᶠ as Heqv_vl Heqv_vₓ Heqv_qₖ / Heqv_vₓ Heqv_qₖ vₓᴮ qₖᴮ:
-          (map erase_val' vlᴮ)
+    rem - vsᶠ vₓᶠ qₖᶠ as Heqv_vs Heqv_vₓ Heqv_qₖ / Heqv_vₓ Heqv_qₖ vₓᴮ qₖᴮ:
+          (map erase_val' vsᴮ)
           (erase_val' vₓᴮ)
           (erase_exc qₖᴮ).
     erewrite length_map_erase_val_eq in *.
-          2-4: exa - Heqv_vl.
-          clr - Heqv_vl vlᴮ.
+          2-4: exa - Heqv_vs.
+          clr - Heqv_vs vsᴮ.
     (* #3 Split Expression List: pose/destruct/subst *)
     psc - length_lt_split_middle as Hsplit:
-          Val Exp vlᶠ elᶠ Hlen.
-    des - Hsplit as [el₁ᶠ [eₖᶠ [el₂ᶠ [Hel Hlen]]]].
+          Val Exp vsᶠ esᶠ Hlen.
+    des - Hsplit as [es₁ᶠ [eₖᶠ [es₂ᶠ [Hes Hlen]]]].
     sbt.
     (* #4 Simplify Hypothesis: *)
     rwr - Hlen in IHFse_qₖ.
     smp - IHFse_qₖ.
     rwr - nth_middle in IHFse_qₖ.
     (* #5 Destruct on Expression List and Solve Empty Branch: destruct *)
-    des - el₁ᶠ as [| e₁ᶠ el₁ᶠ].
+    des - es₁ᶠ as [| e₁ᶠ es₁ᶠ].
     { (* - Empty List Branch *)
           clr - IHFse_nth eₓᶠ vₓᶠ.
           (* #5.1 Both List Empty: apply/subst/simpl *)
@@ -1338,29 +1375,29 @@ Section ETuple.
           step.
     } (* - Cons List Branch *)
     (* #6 Both List Cons: destruct + inversion/subst *)
-    des - vlᶠ as [| v₁ᶠ vlᶠ]:
+    des - vsᶠ as [| v₁ᶠ vsᶠ]:
           ivs - Hlen.
     (* #7 Pose Nth Cons Theorem: rewrite/pose/destruct *)
-    rewrite cons_app with (l := el₁ᶠ) in IHFse_nth.
+    rewrite cons_app with (l := es₁ᶠ) in IHFse_nth.
     rwl - app_assoc in IHFse_nth.
     do 2 rwl - cons_app in IHFse_nth.
     psc - fs_eval_nth_cons as IHFse_nth_cons:
-          e₁ᶠ (el₁ᶠ ++ eₖᶠ :: el₂ᶠ) eₓᶠ v₁ᶠ vlᶠ vₓᶠ IHFse_nth.
+          e₁ᶠ (es₁ᶠ ++ eₖᶠ :: es₂ᶠ) eₓᶠ v₁ᶠ vsᶠ vₓᶠ IHFse_nth.
     des - IHFse_nth_cons as [IHFse_v₁ IHFse_nth].
     (* #8 Pose From Nth to Result: apply/pose/simple *)
-    app - length_cons in Hlen.
+    app - length_cons_eq in Hlen.
     pose proof fs_eval_nth_to_partial
-          ITuple el₁ᶠ eₖᶠ el₂ᶠ eₓᶠ [] v₁ᶠ vlᶠ vₓᶠ Hlen IHFse_nth
-          as IHFse_vl.
+          ITuple es₁ᶠ eₖᶠ es₂ᶠ eₓᶠ [] v₁ᶠ vsᶠ vₓᶠ Hlen IHFse_nth
+          as IHFse_vs.
     smp / Hlen IHFse_nth eₓᶠ vₓᶠ.
     (* #9 Destruct Inductive Hypothesis: destruct *)
     des - IHFse_v₁ as [k_v₁ [_       Hstp_v₁]].
-    des - IHFse_vl as [k_vl          Hstp_vl].
+    des - IHFse_vs as [k_vs          Hstp_vs].
     des - IHFse_qₖ as [k_qₖ [Hscp_qₖ Hstp_qₖ]].
     (* #10 FrameStack Evaluation: open/step *)
     open / Hscp_qₖ.
     step - Hstp_v₁ / e₁ᶠ k_v₁.
-    step - Hstp_vl / el₁ᶠ k_vl.
+    step - Hstp_vs / es₁ᶠ k_vs.
     step - Hstp_qₖ / k_qₖ.
     step.
   Qed.
@@ -1381,34 +1418,46 @@ Section EMap.
 
 
 
+(*
+Hlen_k : ˡ|eesᴮ| = ˡ|ᵏvsᴮ|
+Hlen_v : ˡ|eesᴮ| = ˡ|ᵛvsᴮ|
+Hmake : make_value_map ᵏvsᴮ ᵛvsᴮ = (ᵏvsᴮ, ᵛvsᴮ)
+IHFse_nth :
+  ∀ i : nat,
+    i < ˡ|make_map_exps eesᴮ|
+    → ⟨ [], ᴱ′(δₑᶠ(nth i (make_map_exps eesᴮ) eₓᴮ ⇓ Γ)) ⟩ -->*
+      ᵛˢ′(δᵥₗᶠ([nth i (make_map_vals ᵏvsᴮ ᵛvsᴮ) vₓᴮ]))
+______________________________________(1/1)
+⟨ [], ᴱ′(δₑᶠ(ᵉ∼{eesᴮ}∼ᴮ ⇓ Γ)) ⟩ -->* ᵛˢ′(δᵥₗᶠ([ᵛ∼{combine ᵏvsᴮ ᵛvsᴮ}∼ᴮ]))
+*)
   Theorem eq_bsfs_emap_to_vmap :
-    forall Γ e₂lᴮ eₓᴮ ᵏvlᴮ ᵛvlᴮ vₓᴮ,
-        length e₂lᴮ = length ᵏvlᴮ
-    ->  length e₂lᴮ = length ᵛvlᴮ
-    ->  make_value_map ᵏvlᴮ ᵛvlᴮ = (ᵏvlᴮ, ᵛvlᴮ)
+    forall Γ eesᴮ eₓᴮ ᵏvsᴮ ᵛvsᴮ vₓᴮ,
+        length eesᴮ = length ᵏvsᴮ
+    ->  length eesᴮ = length ᵛvsᴮ
+    ->  make_value_map ᵏvsᴮ ᵛvsᴮ = (ᵏvsᴮ, ᵛvsᴮ)
     ->  (forall i,
-            i < length (make_map_exps e₂lᴮ)
-        ->  ⟨ [], erase_names Γ (nth i (make_map_exps e₂lᴮ) eₓᴮ) ⟩ -->*
-                  erase_valseq [nth i (make_map_vals ᵏvlᴮ ᵛvlᴮ) vₓᴮ])
-    ->  ⟨ [], erase_names Γ (EMap e₂lᴮ) ⟩ -->*
-              erase_valseq [VMap (combine ᵏvlᴮ ᵛvlᴮ)].
+            i < length (make_map_exps eesᴮ)
+        ->  ⟨ [], erase_names Γ (nth i (make_map_exps eesᴮ) eₓᴮ) ⟩ -->*
+                  erase_valseq [nth i (make_map_vals ᵏvsᴮ ᵛvsᴮ) vₓᴮ])
+    ->  ⟨ [], erase_names Γ (EMap eesᴮ) ⟩ -->*
+              erase_valseq [VMap (combine ᵏvsᴮ ᵛvsᴮ)].
   Proof.
-    itr - Γ e₂lᴮ eₓᴮ ᵏvlᴮ ᵛvlᴮ vₓᴮ Hlen_k Hlen_v Hmake IHFse_nth.
+    itr - Γ eesᴮ eₓᴮ ᵏvsᴮ ᵛvsᴮ vₓᴮ Hlen_k Hlen_v Hmake IHFse_nth.
     (* #1 Rewrite Combine Keys-Vals Theorem: rewrite/symmetry/pose/destruct *)
     rwr - make_map_exps_flatten_list_eq in *.
     sym - Hlen_k Hlen_v.
     pose proof length_match2 _ _ _ _ _ _ Hlen_k Hlen_v as Hlen.
-    pse - combine_key_and_val_lists as Hcomb: ᵏvlᴮ ᵛvlᴮ Hlen Hmake.
-    des - Hcomb as [v₂lᴮ [Hᵏvl [Hᵛvl [Hv₂l Hflat]]]].
-    cwr - Hv₂l Hflat Hᵏvl Hᵛvl / Hlen Hlen_v Hmake ᵏvlᴮ ᵛvlᴮ;
+    pse - combine_key_and_val_lists as Hcomb: ᵏvsᴮ ᵛvsᴮ Hlen Hmake.
+    des - Hcomb as [vvsᴮ [Hᵏvs [Hᵛvs [Hvvs Hflat]]]].
+    cwr - Hvvs Hflat Hᵏvs Hᵛvs / Hlen Hlen_v Hmake ᵏvsᴮ ᵛvsᴮ;
           ren - Hlen: Hlen_k.
     rwl - length_map_fst in Hlen.
     rwr - length_flatten_both_eq in Hlen.
     rwl - Hlen in IHFse_nth.
     (* #2 Unfold Converters: pose/rewrite/simpl/unfold/mvr *)
-    pose proof flatten_deflatten e₂lᴮ as He₂l.
-    pose proof flatten_deflatten v₂lᴮ as Hv₂l.
-    cwl - He₂l Hv₂l.
+    pose proof flatten_deflatten eesᴮ as Hees.
+    pose proof flatten_deflatten vvsᴮ as Hvvs.
+    cwl - Hees Hvvs.
     smp *.
     ufl - erase_names in *.
     do 3 rwr - deflatten_map.
@@ -1422,34 +1471,34 @@ Section EMap.
     rem - ξ as Heqv_ξ / Heqv_ξ Γ:
           (list_subst (map erase_val' Γ.vals) idsubst).
     psc - fs_eval_nth_map_erase_forall as IHFse_nth':
-          σ ξ (flatten_list e₂lᴮ) eₓᴮ (flatten_list v₂lᴮ) vₓᴮ IHFse_nth;
+          σ ξ (flatten_list eesᴮ) eₓᴮ (flatten_list vvsᴮ) vₓᴮ IHFse_nth;
           ren - IHFse_nth: IHFse_nth'.
     do 2 rwr - flatten_map in *.
       (* Expressions *)
-    rem - e₂lᶠ eₓᶠ as Heqv_e₂l Heqv_eₓ / Heqv_eₓ eₓᴮ:
-          (map (fun '(x, y) => ((erase_exp σ x).[ξ], (erase_exp σ y).[ξ])) e₂lᴮ)
+    rem - eesᶠ eₓᶠ as Heqv_ees Heqv_eₓ / Heqv_eₓ eₓᴮ:
+          (map (fun '(x, y) => ((erase_exp σ x).[ξ], (erase_exp σ y).[ξ])) eesᴮ)
           ((erase_exp σ eₓᴮ).[ξ]).
     erewrite length_map_erase_exp_flatten_eq in *.
-          2: exa - Heqv_e₂l.
-          clr - Heqv_e₂l e₂lᴮ σ ξ.
+          2: exa - Heqv_ees.
+          clr - Heqv_ees eesᴮ σ ξ.
       (* Values *)
-    rem - v₂lᶠ vₓᶠ as Heqv_v₂l Heqv_vₓ / Heqv_vₓ vₓᴮ:
-          (map (fun '(x, y) => (erase_val' x, erase_val' y)) v₂lᴮ)
+    rem - vvsᶠ vₓᶠ as Heqv_vvs Heqv_vₓ / Heqv_vₓ vₓᴮ:
+          (map (fun '(x, y) => (erase_val' x, erase_val' y)) vvsᴮ)
           (erase_val' vₓᴮ).
     erewrite length_map_erase_val_flatten_eq in *.
-          2-3: exa - Heqv_v₂l.
-          clr - Heqv_v₂l v₂lᴮ.
+          2-3: exa - Heqv_vvs.
+          clr - Heqv_vvs vvsᴮ.
     (* #4 Flatten-Deflatten: pose/rewrite *)
-    pose proof flatten_deflatten e₂lᶠ as He₂l.
-    pose proof flatten_deflatten v₂lᶠ as Hv₂l.
-    cwr - He₂l Hv₂l.
+    pose proof flatten_deflatten eesᶠ as Hees.
+    pose proof flatten_deflatten vvsᶠ as Hvvs.
+    cwr - Hees Hvvs.
     (* #5 Scope From Nth: pose *)
     pse - fs_eval_nth_to_scope as Hscp':
-          (flatten_list e₂lᶠ) eₓᶠ (flatten_list v₂lᶠ) vₓᶠ Hlen IHFse_nth.
+          (flatten_list eesᶠ) eₓᶠ (flatten_list vvsᶠ) vₓᶠ Hlen IHFse_nth.
     psc - scope_list_to_map as Hscp:
-          v₂lᶠ Hscp'.
+          vvsᶠ Hscp'.
     (* #6 Destruct on Expression List and Solve Empty Branch: destruct *)
-    des - e₂lᶠ as [| [ᵏe₁ᶠ ᵛe₁ᶠ] e₂lᶠ].
+    des - eesᶠ as [| [ᵏe₁ᶠ ᵛe₁ᶠ] eesᶠ].
     { (* - Empty List Branch *)
           clr - IHFse_nth Hscp eₓᶠ vₓᶠ.
           (* #6.1 Both List Empty: rewrite/apply/subst *)
@@ -1461,43 +1510,43 @@ Section EMap.
           step.
     } (* - Cons List Branch *)
     (* #7 Both List Cons: destruct + inversion/subst *)
-    des - v₂lᶠ as [| [ᵏv₁ᶠ ᵛv₁ᶠ] v₂lᶠ]:
+    des - vvsᶠ as [| [ᵏv₁ᶠ ᵛv₁ᶠ] vvsᶠ]:
           ivs - Hlen.
     (* #8 Pose Nth Cons Theorem: pose/destruct *)
     do 2 rwr - flatten_cons in *.
     psc - fs_eval_nth_cons as IHFse_nth_cons:
-          ᵏe₁ᶠ (ᵛe₁ᶠ :: flatten_list e₂lᶠ) eₓᶠ
-          ᵏv₁ᶠ (ᵛv₁ᶠ :: flatten_list v₂lᶠ) vₓᶠ
+          ᵏe₁ᶠ (ᵛe₁ᶠ :: flatten_list eesᶠ) eₓᶠ
+          ᵏv₁ᶠ (ᵛv₁ᶠ :: flatten_list vvsᶠ) vₓᶠ
           IHFse_nth.
     des - IHFse_nth_cons as [IHFse_ᵏv₁ IHFse_nth].
     psc - fs_eval_nth_cons as IHFse_nth_cons:
-          ᵛe₁ᶠ (flatten_list e₂lᶠ) eₓᶠ
-          ᵛv₁ᶠ (flatten_list v₂lᶠ) vₓᶠ
+          ᵛe₁ᶠ (flatten_list eesᶠ) eₓᶠ
+          ᵛv₁ᶠ (flatten_list vvsᶠ) vₓᶠ
           IHFse_nth.
     des - IHFse_nth_cons as [IHFse_ᵛv₁ IHFse_nth].
     (* #9 Pose From Nth to Result: apply/pose/destruct/rewrite *)
-    do 2 app - length_cons in Hlen.
+    do 2 app - length_cons_eq in Hlen.
     pose proof create_result_imap
-          ᵏv₁ᶠ ᵛv₁ᶠ v₂lᶠ [] as Hcrt.
+          ᵏv₁ᶠ ᵛv₁ᶠ vvsᶠ [] as Hcrt.
     pse - all_fsval_is_wfm as Hwfm:
-          (Syntax.VMap ((ᵏv₁ᶠ, ᵛv₁ᶠ) :: v₂lᶠ)).
+          (Syntax.VMap ((ᵏv₁ᶠ, ᵛv₁ᶠ) :: vvsᶠ)).
     des - Hwfm as [Hwfm _].
     cwl - Hwfm in Hcrt.
     pose proof fs_eval_nth_to_result
-          IMap (flatten_list e₂lᶠ) eₓᶠ [ᵏv₁ᶠ] ᵛv₁ᶠ (flatten_list v₂lᶠ) vₓᶠ
-          (RValSeq [Syntax.VMap ((ᵏv₁ᶠ, ᵛv₁ᶠ) :: v₂lᶠ)]) [] []
+          IMap (flatten_list eesᶠ) eₓᶠ [ᵏv₁ᶠ] ᵛv₁ᶠ (flatten_list vvsᶠ) vₓᶠ
+          (RValSeq [Syntax.VMap ((ᵏv₁ᶠ, ᵛv₁ᶠ) :: vvsᶠ)]) [] []
           Hlen Hcrt IHFse_nth
-          as IHFse_v₂l;
+          as IHFse_vvs;
           clr - Hlen Hcrt IHFse_nth eₓᶠ vₓᶠ.
     (* #10 Destruct Inductive Hypothesis: destruct *)
     des - IHFse_ᵏv₁ as [k_ᵏv₁ [_ Hstp_ᵏv₁]].
     des - IHFse_ᵛv₁ as [k_ᵛv₁ [_ Hstp_ᵛv₁]].
-    des - IHFse_v₂l as [k_v₂l    Hstp_v₂l].
+    des - IHFse_vvs as [k_vvs    Hstp_vvs].
     (* #11 FrameStack Evaluation: open/step *)
     open / Hscp.
     step - Hstp_ᵏv₁ / ᵏe₁ᶠ k_ᵏv₁.
     step - Hstp_ᵛv₁ / ᵛe₁ᶠ k_ᵛv₁.
-    step - Hstp_v₂l.
+    step - Hstp_vvs.
   Qed.
 
 
@@ -1505,41 +1554,54 @@ Section EMap.
 
 
 
+(*
+Hlen : k < 2 * ˡ|eesᴮ|
+Hlen_k : ˡ|ᵏvsᴮ| = k `div` 2 + k % 2
+Hlen_v : ˡ|ᵛvsᴮ| = k `div` 2
+IHFse_nth :
+  ∀ i : nat,
+    i < k
+    → ⟨ [], ᴱ′(δₑᶠ(nth i (make_map_exps eesᴮ) eₓᴮ ⇓ Γ)) ⟩ -->*
+      ᵛˢ′(δᵥₗᶠ([nth i (make_map_vals ᵏvsᴮ ᵛvsᴮ) vₓᴮ]))
+IHFse_qₖ₂ : ⟨ [], ᴱ′(δₑᶠ(nth k (make_map_exps eesᴮ) eₓᴮ ⇓ Γ)) ⟩ -->* δᶠ(qₖ₂ᴮ ↦)
+______________________________________(1/1)
+⟨ [], ᴱ′(δₑᶠ(ᵉ∼{eesᴮ}∼ᴮ ⇓ Γ)) ⟩ -->* ᵉˣᶜ′(δₓᶠ(qₖ₂ᴮ))
+*)
   Theorem eq_bsfs_emap_to_exception :
-    forall Γ e₂lᴮ eₓᴮ ᵏvlᴮ ᵛvlᴮ vₓᴮ qₖ₂ᴮ k,
-        k < 2 * length e₂lᴮ
-    ->  length ᵏvlᴮ = k / 2 + k mod 2
-    ->  length ᵛvlᴮ = k / 2
+    forall Γ eesᴮ eₓᴮ ᵏvsᴮ ᵛvsᴮ vₓᴮ qₖ₂ᴮ k,
+        k < 2 * length eesᴮ
+    ->  length ᵏvsᴮ = k / 2 + k mod 2
+    ->  length ᵛvsᴮ = k / 2
     ->  (forall i,
             i < k
-        ->  ⟨ [], erase_names Γ (nth i (make_map_exps e₂lᴮ) eₓᴮ) ⟩ -->* 
-                  erase_valseq [nth i (make_map_vals ᵏvlᴮ ᵛvlᴮ) vₓᴮ])
-    ->  ⟨ [], erase_names Γ (nth k (make_map_exps e₂lᴮ) eₓᴮ) ⟩ -->*
+        ->  ⟨ [], erase_names Γ (nth i (make_map_exps eesᴮ) eₓᴮ) ⟩ -->* 
+                  erase_valseq [nth i (make_map_vals ᵏvsᴮ ᵛvsᴮ) vₓᴮ])
+    ->  ⟨ [], erase_names Γ (nth k (make_map_exps eesᴮ) eₓᴮ) ⟩ -->*
               erase_result (inr qₖ₂ᴮ)
-    ->  ⟨ [], erase_names Γ (EMap e₂lᴮ) ⟩ -->*
+    ->  ⟨ [], erase_names Γ (EMap eesᴮ) ⟩ -->*
               erase_exc qₖ₂ᴮ.
   Proof.
-    itr - Γ e₂lᴮ eₓᴮ ᵏvlᴮ ᵛvlᴮ vₓᴮ qₖ₂ᴮ k
+    itr - Γ eesᴮ eₓᴮ ᵏvsᴮ ᵛvsᴮ vₓᴮ qₖ₂ᴮ k
           Hlen Hlen_k Hlen_v IHFse_nth IHFse_qₖ₂.
     (* #1 Rewrite Combine Keys-Vals Theorem: rewrite/pose/destruct/apply *)
     rwr - make_map_exps_flatten_list_eq in *.
     pse - combine_key_and_val_exc as Hcomb:
-          ᵏvlᴮ ᵛvlᴮ k Hlen_k Hlen_v.
-    des - Hcomb as [v₂lᴮ [vlᴮ [Hlen_v₂l [Hlen_vl [Hᵏvl [Hᵛvl Hflat]]]]]].
-    cwr - Hflat Hᵏvl Hᵛvl / Hlen_k Hlen_v ᵏvlᴮ ᵛvlᴮ.
+          ᵏvsᴮ ᵛvsᴮ k Hlen_k Hlen_v.
+    des - Hcomb as [vvsᴮ [vsᴮ [Hlen_vvs [Hlen_vs [Hᵏvs [Hᵛvs Hflat]]]]]].
+    cwr - Hflat Hᵏvs Hᵛvs / Hlen_k Hlen_v ᵏvsᴮ ᵛvsᴮ.
     pse - kmod2length_combined as Hlen_comb:
-          Value v₂lᴮ vlᴮ k Hlen_v₂l Hlen_vl;
-          clr - Hlen_v₂l.
-    psc - kmod2list_is_either_empty_or_single as Hvl:
-          Value vlᴮ k Hlen_vl.
-    app - erase_val_empty_or_single_also in Hvl.
+          Value vvsᴮ vsᴮ k Hlen_vvs Hlen_vs;
+          clr - Hlen_vvs.
+    psc - kmod2list_is_either_empty_or_single as Hvs:
+          Value vsᴮ k Hlen_vs.
+    app - erase_val_empty_or_single_also in Hvs.
     cwl - Hlen_comb / k.
     rwr - Nat.mul_comm in Hlen.
     rewrite <- length_flatten_list in Hlen.
     app - length_app_le in Hlen.
     (* #2 Unfold Converters: pose/rewrite/simpl/unfold *)
-    pose proof flatten_deflatten e₂lᴮ as He₂l.
-    cwl - He₂l.
+    pose proof flatten_deflatten eesᴮ as Hees.
+    cwl - Hees.
     smp *.
     ufl - erase_names in *.
     do 2 rwr - deflatten_map.
@@ -1552,43 +1614,43 @@ Section EMap.
     rem - ξ as Heqv_ξ / Heqv_ξ Γ:
           (list_subst (map erase_val' Γ.vals) idsubst).
     psc - fs_eval_nth_map_erase_forall as IHFse_nth':
-          σ ξ (flatten_list e₂lᴮ) eₓᴮ (flatten_list v₂lᴮ ++ vlᴮ) vₓᴮ IHFse_nth;
+          σ ξ (flatten_list eesᴮ) eₓᴮ (flatten_list vvsᴮ ++ vsᴮ) vₓᴮ IHFse_nth;
           ren - IHFse_nth: IHFse_nth'.
     rwr - fs_eval_nth_map_erase_single in IHFse_qₖ₂.
     rwr - map_app in IHFse_nth.
     do 2 rwr - flatten_map in *.
       (* Expressions *)
-    rem - e₂lᶠ eₓᶠ as Heqv_e₂l Heqv_eₓ / Heqv_eₓ eₓᴮ:
-          (map (fun '(x, y) => ((erase_exp σ x).[ξ], (erase_exp σ y).[ξ])) e₂lᴮ)
+    rem - eesᶠ eₓᶠ as Heqv_ees Heqv_eₓ / Heqv_eₓ eₓᴮ:
+          (map (fun '(x, y) => ((erase_exp σ x).[ξ], (erase_exp σ y).[ξ])) eesᴮ)
           ((erase_exp σ eₓᴮ).[ξ]).
     erewrite length_map_erase_exp_flatten_eq in *.
-          2: exa - Heqv_e₂l.
-          clr - Heqv_e₂l e₂lᴮ σ ξ.
+          2: exa - Heqv_ees.
+          clr - Heqv_ees eesᴮ σ ξ.
       (* Values *)
-    rem - v₂lᶠ vlᶠ vₓᶠ qₖ₂ᶠ as Heqv_v₂l Heqv_vl Heqv_vₓ Heqv_qₖ₂
+    rem - vvsᶠ vsᶠ vₓᶠ qₖ₂ᶠ as Heqv_vvs Heqv_vs Heqv_vₓ Heqv_qₖ₂
           / Heqv_vₓ Heqv_qₖ₂ vₓᴮ qₖ₂ᴮ:
-          (map (fun '(x, y) => (erase_val' x, erase_val' y)) v₂lᴮ)
-          (map erase_val' vlᴮ)
+          (map (fun '(x, y) => (erase_val' x, erase_val' y)) vvsᴮ)
+          (map erase_val' vsᴮ)
           (erase_val' vₓᴮ)
           (erase_exc qₖ₂ᴮ).
-    rwr - length_app in *.
+    rewrite length_app in *.
     erewrite length_map_erase_val_flatten_eq in *.
-          2-4: exa - Heqv_v₂l.
-          clr - Heqv_v₂l v₂lᴮ.
+          2-4: exa - Heqv_vvs.
+          clr - Heqv_vvs vvsᴮ.
     erewrite length_map_erase_val_eq in *.
-          2-3: exa - Heqv_vl.
-          clr - Heqv_vl vlᴮ.
-    rwl - length_app in *.
+          2-3: exa - Heqv_vs.
+          clr - Heqv_vs vsᴮ.
+    rewrite <- length_app in *.
     (* #4 Flatten-Deflatten List: pose/rewrite *)
-    pose proof flatten_deflatten e₂lᶠ as He₂l.
-    cwr - He₂l.
+    pose proof flatten_deflatten eesᶠ as Hees.
+    cwr - Hees.
     rwl - length_flatten_both_lt in Hlen.
     (* #5 Split Expression List: pose/destruct/subst/rewrite/simpl *)
     epose proof length_lt_split_middle
-          _ _ v₂lᶠ e₂lᶠ Hlen
+          _ _ vvsᶠ eesᶠ Hlen
           as Hsplit;
           clr - Hlen.
-    des - Hsplit as [e₂l₁ᶠ [[ᵏeₖ₂ᶠ ᵛeₖ₂ᶠ] [e₂l₂ᶠ [Hel Hlen]]]].
+    des - Hsplit as [ees₁ᶠ [[ᵏeₖ₂ᶠ ᵛeₖ₂ᶠ] [ees₂ᶠ [Hes Hlen]]]].
     sbt.
     smp *.
     (* #6 Flatten List: rewrite *)
@@ -1596,7 +1658,7 @@ Section EMap.
     rwr - flatten_app in *.
     rewrite flatten_cons in *.
     (* #6 Destruct Empty or Single: destruct/subst *)
-    des - Hvl as [Hempty | [ᵏvₖ₂ᶠ Hsingle]]; sbt.
+    des - Hvs as [Hempty | [ᵏvₖ₂ᶠ Hsingle]]; sbt.
     * (* +I. Rest is Empty: *)
       (* #I/1 Simplify Hypothesis: rename/rewrite *)
       ren - IHFse_ᵏqₖ₂ ᵏqₖ₂ᶠ: IHFse_qₖ₂ qₖ₂ᶠ.
@@ -1604,7 +1666,7 @@ Section EMap.
       rwr - Hlen in IHFse_ᵏqₖ₂.
       rwr - nth_middle in IHFse_ᵏqₖ₂.
       (* #I/2 Destruct on Expression List and Solve Empty Branch: destruct *)
-      des - e₂l₁ᶠ as [| [ᵏe₁ᶠ ᵛe₁ᶠ] e₂l₁ᶠ].
+      des - ees₁ᶠ as [| [ᵏe₁ᶠ ᵛe₁ᶠ] ees₁ᶠ].
       { (* - Empty List Branch *)
             clr - IHFse_nth eₓᶠ vₓᶠ.
             (* #I/2.1 Both List Empty: rewrite/apply/subst/simpl *)
@@ -1620,70 +1682,70 @@ Section EMap.
             step.
       } (* - Cons List Branch *)
       (* #I/3 Both List Cons: destruct + inversion/subst *)
-      des - v₂lᶠ as [| [ᵏv₁ᶠ ᵛv₁ᶠ] v₂lᶠ]:
+      des - vvsᶠ as [| [ᵏv₁ᶠ ᵛv₁ᶠ] vvsᶠ]:
             ivs - Hlen.
       (* #I/4 Pose Nth Cons Theorem: rewrite/pose/destruct *)
       do 2 rwr - flatten_cons in *.
       do 2 rwl - app_comm_cons in *.
       psc - fs_eval_nth_cons as IHFse_nth_cons:
-            ᵏe₁ᶠ (ᵛe₁ᶠ :: flatten_list e₂l₁ᶠ
-              ++ ᵏeₖ₂ᶠ :: ᵛeₖ₂ᶠ :: flatten_list e₂l₂ᶠ) eₓᶠ
-            ᵏv₁ᶠ (ᵛv₁ᶠ :: flatten_list v₂lᶠ) vₓᶠ
+            ᵏe₁ᶠ (ᵛe₁ᶠ :: flatten_list ees₁ᶠ
+              ++ ᵏeₖ₂ᶠ :: ᵛeₖ₂ᶠ :: flatten_list ees₂ᶠ) eₓᶠ
+            ᵏv₁ᶠ (ᵛv₁ᶠ :: flatten_list vvsᶠ) vₓᶠ
             IHFse_nth.
       des - IHFse_nth_cons as [IHFse_ᵏv₁ IHFse_nth].
       psc - fs_eval_nth_cons as IHFse_nth_cons:
-            ᵛe₁ᶠ (flatten_list e₂l₁ᶠ
-              ++ ᵏeₖ₂ᶠ :: ᵛeₖ₂ᶠ :: flatten_list e₂l₂ᶠ) eₓᶠ
-            ᵛv₁ᶠ (flatten_list v₂lᶠ) vₓᶠ
+            ᵛe₁ᶠ (flatten_list ees₁ᶠ
+              ++ ᵏeₖ₂ᶠ :: ᵛeₖ₂ᶠ :: flatten_list ees₂ᶠ) eₓᶠ
+            ᵛv₁ᶠ (flatten_list vvsᶠ) vₓᶠ
             IHFse_nth.
       des - IHFse_nth_cons as [IHFse_ᵛv₁ IHFse_nth].
       (* #I/5 Pose From Nth to Result: apply/pose/rewrite *)
-      do 2 app - length_cons in Hlen.
+      do 2 app - length_cons_eq in Hlen.
       pose proof fs_eval_nth_to_partial
-            IMap (flatten_list e₂l₁ᶠ) ᵏeₖ₂ᶠ (ᵛeₖ₂ᶠ :: flatten_list e₂l₂ᶠ) eₓᶠ
-            [ᵏv₁ᶠ] ᵛv₁ᶠ (flatten_list v₂lᶠ) vₓᶠ
+            IMap (flatten_list ees₁ᶠ) ᵏeₖ₂ᶠ (ᵛeₖ₂ᶠ :: flatten_list ees₂ᶠ) eₓᶠ
+            [ᵏv₁ᶠ] ᵛv₁ᶠ (flatten_list vvsᶠ) vₓᶠ
             Hlen IHFse_nth
-            as IHFse_v₂l;
+            as IHFse_vvs;
             clr - Hlen IHFse_nth eₓᶠ vₓᶠ.
       rwl - flatten_cons in *.
       rwl - flatten_app in *.
       (* #I/6 Destruct Inductive Hypothesis: destruct *)
       des - IHFse_ᵏv₁  as [k_ᵏv₁   [_         Hstp_ᵏv₁]].
       des - IHFse_ᵛv₁  as [k_ᵛv₁   [_         Hstp_ᵛv₁]].
-      des - IHFse_v₂l  as [k_v₂l              Hstp_v₂l].
+      des - IHFse_vvs  as [k_vvs              Hstp_vvs].
       des - IHFse_ᵏqₖ₂ as [k_ᵏqₖ₂  [Hscp_ᵏqₖ₂ Hstp_ᵏqₖ₂]].
       (* #I/7 FrameStack Evaluation: open/step *)
       open / Hscp_ᵏqₖ₂.
       step - Hstp_ᵏv₁  / ᵏe₁ᶠ  k_ᵏv₁.
       step - Hstp_ᵛv₁  / ᵛe₁ᶠ  k_ᵛv₁.
-      step - Hstp_v₂l  / e₂l₁ᶠ k_v₂l.
+      step - Hstp_vvs  / ees₁ᶠ k_vvs.
       step - Hstp_ᵏqₖ₂ / ᵏeₖ₂ᶠ k_ᵏqₖ₂.
       step.
     * (* +II. Rest is Single: *)
       (* #II/1 Simplify Hypothesis: rename/rewrite *)
       ren - IHFse_ᵛqₖ₂ ᵛqₖ₂ᶠ: IHFse_qₖ₂ qₖ₂ᶠ.
-      rwr - length_app in *.
+      rewrite length_app in *.
       rwr - Hlen in *.
       rewrite cons_app with (x := ᵏeₖ₂ᶠ) in IHFse_ᵛqₖ₂.
       pose proof length_app_end_any
-            _ _ _ (flatten_list e₂l₁ᶠ) ᵏvₖ₂ᶠ ᵏeₖ₂ᶠ
+            _ _ _ (flatten_list ees₁ᶠ) ᵏvₖ₂ᶠ ᵏeₖ₂ᶠ
             as Hlen_swap.
       rwr - Hlen_swap in *.
-      rwl - length_app in *.
+      rewrite <- length_app in *.
       rwr - app_assoc in *.
       rwr - nth_middle in IHFse_ᵛqₖ₂.
-      rwr - length_app in IHFse_nth.
+      rewrite length_app in IHFse_nth.
       pse - length_add_end_le as Hle:
-            Exp (flatten_list e₂l₁ᶠ) ᵏeₖ₂ᶠ.
+            Exp (flatten_list ees₁ᶠ) ᵏeₖ₂ᶠ.
       spc + IHFse_nth as IHFse_ᵏvₖ₂:
-            (length (flatten_list e₂l₁ᶠ)) Hle.
+            (length (flatten_list ees₁ᶠ)) Hle.
       rwr - nth_middle in IHFse_ᵏvₖ₂.
-      rwl - length_app in IHFse_nth.
+      rewrite <- length_app in IHFse_nth.
       cwl - Hlen_swap in IHFse_nth.
       rwl - Hlen in IHFse_nth.
-      rwl - length_app in IHFse_nth.
+      rewrite <- length_app in IHFse_nth.
       (* #II/2 Destruct on Expression List and Solve Empty Branch: destruct *)
-      des - e₂l₁ᶠ as [| [ᵏe₁ᶠ ᵛe₁ᶠ] e₂l₁ᶠ].
+      des - ees₁ᶠ as [| [ᵏe₁ᶠ ᵛe₁ᶠ] ees₁ᶠ].
       { (* - Empty List Branch *)
             clr - IHFse_nth eₓᶠ.
             (* #II/2.1 Both List Empty: rewrite/apply/subst/simpl *)
@@ -1702,51 +1764,51 @@ Section EMap.
       } (* - Cons List Branch *)
       (* #I/3 Both List Cons: destruct + inversion/subst *)
       clr - IHFse_ᵏvₖ₂.
-      des - v₂lᶠ as [| [ᵏv₁ᶠ ᵛv₁ᶠ] v₂lᶠ]:
+      des - vvsᶠ as [| [ᵏv₁ᶠ ᵛv₁ᶠ] vvsᶠ]:
             ivs - Hlen.
       (* #I/4 Pose Nth Cons Theorem: rewrite/pose/destruct *)
       do 2 rwr - flatten_cons in *.
       do 2 rwl - app_comm_cons in *.
       psc - fs_eval_nth_cons as IHFse_nth_cons:
-            ᵏe₁ᶠ (ᵛe₁ᶠ :: flatten_list e₂l₁ᶠ
-              ++ ᵏeₖ₂ᶠ :: ᵛeₖ₂ᶠ :: flatten_list e₂l₂ᶠ) eₓᶠ
-            ᵏv₁ᶠ (ᵛv₁ᶠ :: flatten_list v₂lᶠ ++ [ᵏvₖ₂ᶠ]) vₓᶠ
+            ᵏe₁ᶠ (ᵛe₁ᶠ :: flatten_list ees₁ᶠ
+              ++ ᵏeₖ₂ᶠ :: ᵛeₖ₂ᶠ :: flatten_list ees₂ᶠ) eₓᶠ
+            ᵏv₁ᶠ (ᵛv₁ᶠ :: flatten_list vvsᶠ ++ [ᵏvₖ₂ᶠ]) vₓᶠ
             IHFse_nth.
       des - IHFse_nth_cons as [IHFse_ᵏv₁ IHFse_nth].
       psc - fs_eval_nth_cons as IHFse_nth_cons:
-            ᵛe₁ᶠ (flatten_list e₂l₁ᶠ
-              ++ ᵏeₖ₂ᶠ :: ᵛeₖ₂ᶠ :: flatten_list e₂l₂ᶠ) eₓᶠ
-            ᵛv₁ᶠ (flatten_list v₂lᶠ ++ [ᵏvₖ₂ᶠ]) vₓᶠ
+            ᵛe₁ᶠ (flatten_list ees₁ᶠ
+              ++ ᵏeₖ₂ᶠ :: ᵛeₖ₂ᶠ :: flatten_list ees₂ᶠ) eₓᶠ
+            ᵛv₁ᶠ (flatten_list vvsᶠ ++ [ᵏvₖ₂ᶠ]) vₓᶠ
             IHFse_nth.
       des - IHFse_nth_cons as [IHFse_ᵛv₁ IHFse_nth].
       (* #I/5 Pose From Nth to Result: apply/simply/pose/rewrite *)
-      app - length_cons in Hlen.
+      app - length_cons_eq in Hlen.
       smp - Hlen.
       psc - length_succ_add_end as Hlen':
-            Val Exp (flatten_list v₂lᶠ) ᵏvₖ₂ᶠ (flatten_list e₂l₁ᶠ) ᵏeₖ₂ᶠ Hlen;
+            Val Exp (flatten_list vvsᶠ) ᵏvₖ₂ᶠ (flatten_list ees₁ᶠ) ᵏeₖ₂ᶠ Hlen;
             ren - Hlen: Hlen'.
       rewrite cons_app with (x := ᵏeₖ₂ᶠ) in IHFse_nth.
       rwr - app_assoc in IHFse_nth.
       pose proof fs_eval_nth_to_partial
-            IMap (flatten_list e₂l₁ᶠ ++ [ᵏeₖ₂ᶠ]) ᵛeₖ₂ᶠ (flatten_list e₂l₂ᶠ) eₓᶠ
-            [ᵏv₁ᶠ] ᵛv₁ᶠ (flatten_list v₂lᶠ ++ [ᵏvₖ₂ᶠ]) vₓᶠ
+            IMap (flatten_list ees₁ᶠ ++ [ᵏeₖ₂ᶠ]) ᵛeₖ₂ᶠ (flatten_list ees₂ᶠ) eₓᶠ
+            [ᵏv₁ᶠ] ᵛv₁ᶠ (flatten_list vvsᶠ ++ [ᵏvₖ₂ᶠ]) vₓᶠ
             Hlen IHFse_nth
-            as IHFse_v₂l;
+            as IHFse_vvs;
             clr - Hlen IHFse_nth eₓᶠ vₓᶠ.
-      rwl - app_assoc in IHFse_v₂l.
-      smp - IHFse_v₂l.
-      rwl - flatten_cons in IHFse_v₂l.
-      rwl - flatten_app in IHFse_v₂l.
+      rwl - app_assoc in IHFse_vvs.
+      smp - IHFse_vvs.
+      rwl - flatten_cons in IHFse_vvs.
+      rwl - flatten_app in IHFse_vvs.
       (* #I/6 Destruct Inductive Hypothesis: destruct *)
       des - IHFse_ᵏv₁  as [k_ᵏv₁   [_         Hstp_ᵏv₁]].
       des - IHFse_ᵛv₁  as [k_ᵛv₁   [_         Hstp_ᵛv₁]].
-      des - IHFse_v₂l  as [k_v₂l              Hstp_v₂l].
+      des - IHFse_vvs  as [k_vvs              Hstp_vvs].
       des - IHFse_ᵛqₖ₂ as [k_ᵛqₖ₂  [Hscp_ᵛqₖ₂ Hstp_ᵛqₖ₂]].
       (* #I/7 FrameStack Evaluation: open/step *)
       open / Hscp_ᵛqₖ₂.
       step - Hstp_ᵏv₁  / ᵏe₁ᶠ  k_ᵏv₁.
       step - Hstp_ᵛv₁  / ᵛe₁ᶠ  k_ᵛv₁.
-      step - Hstp_v₂l  / e₂l₁ᶠ k_v₂l.
+      step - Hstp_vvs  / ees₁ᶠ k_vvs.
       step - Hstp_ᵛqₖ₂ / ᵛeₖ₂ᶠ k_ᵛqₖ₂.
       step.
   Qed.
@@ -2529,6 +2591,11 @@ Section EqBsFs.
 
 
 
+(*
+B : | Γ, modules, own_module, id, eᴮ, eff | -e> | id', rᴮ, eff' |
+______________________________________(1/1)
+⟨ [], ᴱ′(δₑᶠ(eᴮ ⇓ Γ)) ⟩ -->* δᶠ(rᴮ)
+*)
   Theorem eq_bsfs :
     forall Γ modules own_module id id' eᴮ rᴮ eff eff',
         (eval_expr Γ modules own_module id eᴮ eff id' rᴮ eff')
@@ -2682,89 +2749,89 @@ Section EqBsFs.
         (* -6.1.1 valseq: *)
           1: {
             clr - modules own_module id id' ids eff eff1 eff' H0 H1 H2 H4 H5.
-            ren - el vl Hlen IHFse_nth:
+            ren - es vs Hlen IHFse_nth:
                   exps vals H H3.
             rem - eₓ vₓ as He Hv / He Hv:
                   ErrorExp
                   ErrorValue.
             bse - eq_bsfs_evalues_to_valseq:
-                  Γ el eₓ vl vₓ Hlen IHFse_nth.
+                  Γ es eₓ vs vₓ Hlen IHFse_nth.
           }
         (* -6.1.2 exception: *)
           1:  {
             clr - modules own_module id id' ids eff eff1 eff' H1 H2 H3 B.
-            ren - el vl qₖ Hlen IHFse_nth IHFse_qₖ:
+            ren - es vs qₖ Hlen IHFse_nth IHFse_qₖ:
                   exps vals ex H H4 IHB.
             subst.
             rem - eₓ vₓ as He Hv / He Hv:
                   ErrorExp
                   ErrorValue.
             bse - eq_bsfs_evalues_to_exception:
-                  Γ el eₓ vl vₓ qₖ Hlen IHFse_nth IHFse_qₖ.
+                  Γ es eₓ vs vₓ qₖ Hlen IHFse_nth IHFse_qₖ.
           }
       (* +6.2 ETuple: vtuple/exception *)
         (* -6.2.1 vtuple: *)
           1:  {
             clr - modules own_module id id' ids eff eff1 eff2 H0 H1 H2 H4 H5.
-            ren - el vl Hlen IHFse_nth:
+            ren - es vs Hlen IHFse_nth:
                   exps vals H H3.
             rem - eₓ vₓ as He Hv / He Hv:
                   ErrorExp
                   ErrorValue.
             bse - eq_bsfs_etuple_to_vtuple:
-                  Γ el eₓ vl vₓ Hlen IHFse_nth.
+                  Γ es eₓ vs vₓ Hlen IHFse_nth.
           }
         (* -6.2.2 exception: *)
           7:  {
             clr - modules own_module id id' ids eff eff1 eff2 H1 H2 H3 B.
-            ren - el vl qₖ Hlen IHFse_nth IHFse_qₖ:
+            ren - es vs qₖ Hlen IHFse_nth IHFse_qₖ:
                   exps vals ex H H4 IHB.
             subst.
             rem - eₓ vₓ as He Hv / He Hv:
                   ErrorExp
                   ErrorValue.
             bse - eq_bsfs_etuple_to_exception:
-                  Γ el eₓ vl vₓ qₖ Hlen IHFse_nth IHFse_qₖ.
+                  Γ es eₓ vs vₓ qₖ Hlen IHFse_nth IHFse_qₖ.
           }
       (* +6.3 EMap: vmap/exception *)
         (* -6.3.1 vmap: *)
           6: {
-            ren - e₂l v₂l ᵏvl ᵛvl kvm vvm eff' eff'':
+            ren - ees vvs ᵏvs ᵛvs kvm vvm eff' eff'':
                   l lv kvals vvals kvals' vvals' eff1 eff2.
             ren - Hlen_v Hlen_k Hlen_eff Hlen_id IHFse_nth IHBse_nth:
                   H H0 H1 H2 H4 H3.
             ren - Hmake Hcomb Heq_eff Heq_id:
                   H5 H6 H7 H8.
             pse - map_is_wfm as Hwfm:
-                  Γ modules own_module e₂l ᵏvl ᵛvl kvm vvm v₂l
+                  Γ modules own_module ees ᵏvs ᵛvs kvm vvm vvs
                   eff eff' eff'' ids id id'.
             spe - Hwfm:
                   Hlen_v Hlen_k Hlen_eff Hlen_id
                   IHBse_nth Hmake Hcomb Heq_eff Heq_id;
                   clr - IHBse_nth Hlen_id Hlen_eff Heq_eff Heq_id;
                   clr - modules own_module ids id id' eff eff' eff''.
-            des - Hwfm as [Hᵏvl Hᵛvl].
-            cwl - Hᵏvl Hᵛvl in *.
+            des - Hwfm as [Hᵏvs Hᵛvs].
+            cwl - Hᵏvs Hᵛvs in *.
             subst exps vals.
             subst.
             rem - eₓ vₓ as He Hv / He Hv:
                   ErrorExp
                   ErrorValue.
             bse - eq_bsfs_emap_to_vmap:
-                  Γ e₂l eₓ ᵏvl ᵛvl vₓ Hlen_k Hlen_v Hmake IHFse_nth.
+                  Γ ees eₓ ᵏvs ᵛvs vₓ Hlen_k Hlen_v Hmake IHFse_nth.
           }
         (* -6.3.2 exception: *)
           19: {
             clr - modules own_module eff eff1 eff2 id id' ids H2 H3 H4 B.
-            ren - e₂l qₖ k ᵏvl ᵛvl Hlen_e₂l Hlen_k Hlen_v IHFse_nth IHFse_qₖ:
+            ren - ees qₖ k ᵏvs ᵛvs Hlen_ees Hlen_k Hlen_v IHFse_nth IHFse_qₖ:
                   l ex i kvals vvals H H1 H0 H5 IHB.
             subst exps vals.
             rem - eₓ vₓ as He Hv / He Hv:
                   ErrorExp
                   ErrorValue.
             bse - eq_bsfs_emap_to_exception:
-                  Γ e₂l eₓ ᵏvl ᵛvl vₓ qₖ k
-                  Hlen_e₂l Hlen_k Hlen_v IHFse_nth IHFse_qₖ.
+                  Γ ees eₓ ᵏvs ᵛvs vₓ qₖ k
+                  Hlen_ees Hlen_k Hlen_v IHFse_nth IHFse_qₖ.
           }
     (* #7 Compounds: EPrimOp/EApply/ECall/ECase *)
       (* +7.1 EPrimOp: result/exception *)
